feat: new evaluator invariant

GroupoidModel/Syntax/Typechecker/Value.lean
@@ -1,5 +1,5 @@
+import GroupoidModel.Syntax.GCongr
 import GroupoidModel.Syntax.Injectivity
-import GroupoidModel.Syntax.SubstList
 
 /-! # Values, neutral forms, closures, and evaluation environments
 
@@ -11,6 +11,10 @@ We relate them to the core syntax with `Val.toExpr/Neut.toExpr/Clos.toExpr/sbOfE
 
 /-- Shorthand for `List.length` which is used a lot in this file. -/
 local notation "‖" l "‖" => List.length l
+
+attribute [local grind]
+  EqTp.refl_tp EqTp.symm_tp EqTp.trans_tp
+  EqTm.refl_tm EqTm.symm_tm EqTm.trans_tm
 
 mutual
 /-- Values are produced by the evaluator during NbE.
@@ -57,8 +61,8 @@ because readback is typed, so will have sufficient typing data available. -/
 inductive Val where
   | pi (l l' : Nat) (A : Val) (B : Clos)
   | sigma (l l' : Nat) (A : Val) (B : Clos)
-  | lam (l l' : Nat) (A : Expr) (b : Clos)
-  | pair (l l' : Nat) (B : Expr) (t u : Val)
+  | lam (l l' : Nat) (b : Clos)
+  | pair (l l' : Nat) (t u : Val)
   | univ (l : Nat)
   /- TODO: to make the theory usable,
   we'll need to treat `code` and `el` as eliminators,
@@ -68,17 +72,17 @@ inductive Val where
   | code (A : Val)
   /-- A neutral form. -/
   | neut (n : Neut)
-  deriving Inhabited, Repr, Lean.ToExpr
+  deriving Inhabited
 
 /-- Neutral forms are elimination forms that are 'stuck',
 i.e., contain no β-reducible subterm. -/
 inductive Neut where
   /-- A de Bruijn *level*. -/
   | bvar (i : Nat)
-  | app (l l' : Nat) (B : Expr) (f : Neut) (a : Val)
-  | fst (l l' : Nat) (A B : Expr) (p : Neut)
-  | snd (l l' : Nat) (A B : Expr) (p : Neut)
-  deriving Lean.ToExpr
+  | app (l l' : Nat) (f : Neut) (a : Val)
+  | fst (l l' : Nat) (p : Neut)
+  | snd (l l' : Nat) (p : Neut)
+  deriving Inhabited
 
 /-- Recall that given `Γ.A ⊢ b : B` and a substitution `Δ ⊢ env : Γ`,
 `Δ.A ⊢ b[(env∘↑).v₀] : B[(env∘↑).v₀]`.
@@ -94,369 +98,290 @@ the present variant is a defunctionalization due to Abel. -/
 inductive Clos where
   | mk_tp (Γ : Ctx) (A : Expr) (env : List Val) (B : Expr)
   | mk_tm (Γ : Ctx) (A : Expr) (env : List Val) (b : Expr)
-  deriving Lean.ToExpr
+  deriving Inhabited
 end
 
-/-! ## Values as expressions -/
+/-! ## Relation of values to terms -/
 
 mutual
-variable (d : Nat)
-/-- The expression corresponding to a value well-typed in a context of length `d`. -/
-def Val.toExpr : Val → Expr
-  | .pi l l' A B => .pi l l' A.toExpr B.toExpr
-  | .sigma l l' A B => .sigma l l' A.toExpr B.toExpr
-  | .lam l l' A b => .lam l l' A b.toExpr
-  | .pair l l' B t u => .pair l l' B t.toExpr u.toExpr
-  | .univ l => .univ l
-  | .el a => .el a.toExpr
-  | .code A => .code A.toExpr
-  | .neut n => n.toExpr
-  termination_by v => sizeOf v
-
-/-- The expression corresponding to a neutral form well-typed in a context of length `d`. -/
-def Neut.toExpr : Neut → Expr
-  | .bvar l => .bvar (d - l - 1)
-  | .app l l' B f a => .app l l' B f.toExpr a.toExpr
-  | .fst l l' A B p => .fst l l' A B p.toExpr
-  | .snd l l' A B p => .snd l l' A B p.toExpr
-  termination_by n => sizeOf n
-
-/-- The expression corresponding to a closure
-whose _domain_ is a context of length `d`
-(i.e., `Δ ⊢ env : Γ` where `‖Δ‖ = d`).
-
-Remark: closures are the only kind of value
-that is not fully described by its `Expr` embedding.
-More precisely, the well-typedness of `C.toExpr`
-does not imply that `C` is well-formed.
-This is the only reason why we need `WfVal/…` judgments. -/
-def Clos.toExpr : Clos → Expr
-  | .mk_tp _ _ env B => B.subst (Expr.up <| sbOfEnv env)
-  | .mk_tm _ _ env b => b.subst (Expr.up <| sbOfEnv env)
-  termination_by c => sizeOf c
-
-/-- The substitution corresponding to an evaluation environment
-whose _domain_ is a context of length `d`
-(i.e., `Δ ⊢ env : Γ` where `‖Δ‖ = d`).
-
-See also `sbOfTms`. -/
-def sbOfEnv (env : List Val) (k := 0) : Nat → Expr :=
-  sbOfTms (env.map (·.toExpr)) k
-  termination_by sizeOf env
-end
-
-/-! ## Substitutions from environments -/
-
-@[autosubst]
-theorem sbOfEnv_nil (d) : sbOfEnv d [] = Expr.bvar := by
-  simp [sbOfEnv, autosubst]
-
-@[autosubst]
-theorem sbOfEnv_cons (d t ts k) :
-    sbOfEnv d (t :: ts) k = Expr.snoc (sbOfEnv d ts (k + 1)) (t.toExpr d) := by
-  simp [sbOfEnv, autosubst]
-
-theorem sbOfEnv_get_eq {d ts k i} : i < ts.length → sbOfEnv d ts k i = sbOfEnv d ts 0 i := by
-  intro h
-  unfold sbOfEnv
-  apply sbOfTms_get_eq
-  simp [h]
-
-theorem WfTp.sbOfEnv_irrel {Γ l A ts} (wf : Γ ⊢[l] A) (le : ‖Γ‖ ≤ ‖ts‖) (d k) :
-    A.subst (sbOfEnv d ts k) = A.subst (sbOfEnv d ts 0) := by
-  simp [sbOfEnv, wf.sbOfTms_irrel, le]
-
-theorem WfTm.sbOfEnv_irrel {Γ l A t ts} (wf : Γ ⊢[l] t : A) (le : ‖Γ‖ ≤ ‖ts‖) (d k) :
-     t.subst (sbOfEnv d ts k) = t.subst (sbOfEnv d ts 0) := by
-  simp [sbOfEnv, wf.sbOfTms_irrel, le]
-
-/-! ## Well-formed values -/
-
-mutual
-inductive WfValTp : Ctx → Nat → Val → Prop
-  | pi {Γ A B l l'} :
-    WfValTp Γ l A →
-    WfClosTp Γ l l' (A.toExpr ‖Γ‖) B →
-    WfValTp Γ (max l l') (.pi l l' A B)
-  | sigma {Γ A B l l'} :
-    WfValTp Γ l A →
-    WfClosTp Γ l l' (A.toExpr ‖Γ‖) B →
-    WfValTp Γ (max l l') (.sigma l l' A B)
+inductive ValEqTp : Ctx → Nat → Val → Expr → Prop
+  | pi {Γ vA A vB B l l'} :
+    ValEqTp Γ l vA A →
+    ClosEqTp Γ l l' A vB B →
+    ValEqTp Γ (max l l') (.pi l l' vA vB) (.pi l l' A B)
+  | sigma {Γ vA A vB B l l'} :
+    ValEqTp Γ l vA A →
+    ClosEqTp Γ l l' A vB B →
+    ValEqTp Γ (max l l') (.sigma l l' vA vB) (.sigma l l' A B)
   | univ {Γ l} :
     WfCtx Γ →
     l < univMax →
-    WfValTp Γ (l + 1) (.univ l)
-  | el {Γ a l} :
-    WfValTm Γ (l + 1) a (.univ l) →
-    WfValTp Γ l (.el a)
+    ValEqTp Γ (l + 1) (.univ l) (.univ l)
+  | el {Γ va a l} :
+    ValEqTm Γ (l + 1) va a (.univ l) →
+    ValEqTp Γ l (.el va) (.el a)
+  | conv_tp {Γ vA A A' l} :
+    ValEqTp Γ l vA A →
+    Γ ⊢[l] A ≡ A' →
+    ValEqTp Γ l vA A'
 
 -- Note: no neutral types atm.
 
-inductive WfValTm : Ctx → Nat → Val → Expr → Prop
-  | lam {Γ A B b l l'} :
-    WfClosTm Γ l l' A B b →
-    WfValTm Γ (max l l') (.lam l l' A b) (.pi l l' A B)
-  | pair {Γ A B t u l l'} :
+inductive ValEqTm : Ctx → Nat → Val → Expr → Expr → Prop
+  | lam {Γ A B vb b l l'} :
+    ClosEqTm Γ l l' A B vb b →
+    ValEqTm Γ (max l l') (.lam l l' vb) (.lam l l' A b) (.pi l l' A B)
+  | pair {Γ A B vt t vu u l l'} :
     (A, l) :: Γ ⊢[l'] B →
-    WfValTm Γ l t A →
-    WfValTm Γ l' u (B.subst (t.toExpr ‖Γ‖).toSb) →
-    WfValTm Γ (max l l') (.pair l l' B t u) (.sigma l l' A B)
-  | code {Γ A l} :
+    ValEqTm Γ l vt t A →
+    ValEqTm Γ l' vu u (B.subst t.toSb) →
+    ValEqTm Γ (max l l') (.pair l l' vt vu) (.pair l l' B t u) (.sigma l l' A B)
+  | code {Γ vA A l} :
     l < univMax →
-    WfValTp Γ l A →
-    WfValTm Γ (l + 1) (.code A) (.univ l)
-  | neut_tm {Γ A n l} :
-    WfNeutTm Γ l n A →
-    WfValTm Γ l (.neut n) A
-  | conv_nf {Γ A A' v l} :
-    WfValTm Γ l v A →
+    ValEqTp Γ l vA A →
+    ValEqTm Γ (l + 1) (.code vA) (.code A) (.univ l)
+  | neut_tm {Γ A vn n l} :
+    NeutEqTm Γ l vn n A →
+    ValEqTm Γ l (.neut vn) n A
+  | conv_nf {Γ A A' vt t t' l} :
+    ValEqTm Γ l vt t A →
+    Γ ⊢[l] t ≡ t' : A →
     Γ ⊢[l] A ≡ A' →
-    WfValTm Γ l v A'
+    ValEqTm Γ l vt t' A'
 
-inductive WfNeutTm : Ctx → Nat → Neut → Expr → Prop
+inductive NeutEqTm : Ctx → Nat → Neut → Expr → Expr → Prop
   | bvar {Γ A i l} :
     WfCtx Γ →
     Lookup Γ i A l →
-    WfNeutTm Γ l (.bvar (‖Γ‖ - i - 1)) A
-  | app {Γ A B f a l l'} :
-    WfNeutTm Γ (max l l') f (.pi l l' A B) →
-    WfValTm Γ l a A →
-    WfNeutTm Γ l' (.app l l' B f a) (B.subst (a.toExpr ‖Γ‖).toSb)
-  | fst {Γ A B p l l'} :
-    WfNeutTm Γ (max l l') p (.sigma l l' A B) →
-    WfNeutTm Γ l (.fst l l' A B p) A
-  | snd {Γ A B p l l'} :
-    WfNeutTm Γ (max l l') p (.sigma l l' A B) →
-    WfNeutTm Γ l' (.snd l l' A B p) (B.subst (Expr.fst l l' A B (p.toExpr ‖Γ‖)).toSb)
-  | conv_neut {Γ A A' n l} :
-    WfNeutTm Γ l n A →
+    NeutEqTm Γ l (.bvar (‖Γ‖ - i - 1)) (.bvar i) A
+  | app {Γ A B vf f va a l l'} :
+    NeutEqTm Γ (max l l') vf f (.pi l l' A B) →
+    ValEqTm Γ l va a A →
+    NeutEqTm Γ l' (.app l l' vf va) (.app l l' B f a) (B.subst a.toSb)
+  | fst {Γ A B vp p l l'} :
+    NeutEqTm Γ (max l l') vp p (.sigma l l' A B) →
+    NeutEqTm Γ l (.fst l l' vp) (.fst l l' A B p) A
+  | snd {Γ A B vp p l l'} :
+    NeutEqTm Γ (max l l') vp p (.sigma l l' A B) →
+    NeutEqTm Γ l' (.snd l l' vp) (.snd l l' A B p) (B.subst (Expr.fst l l' A B p).toSb)
+  | conv_neut {Γ A A' vn n n' l} :
+    NeutEqTm Γ l vn n A →
+    Γ ⊢[l] n ≡ n' : A →
     Γ ⊢[l] A ≡ A' →
-    WfNeutTm Γ l n A'
+    NeutEqTm Γ l vn n' A'
 
-/-- `WfClosTp Δ l l' A B` -/
-inductive WfClosTp : Ctx → Nat → Nat → Expr → Clos → Prop
-  | clos_tp {Δ Γ A B Aenv env l l'} :
+/-- `ClosEqTp Δ l l' A vB B` -/
+inductive ClosEqTp : Ctx → Nat → Nat → Expr → Clos → Expr → Prop
+  | clos_tp {Δ Γ A B Aenv env σ l l'} :
+    EnvEqSb Δ env σ Γ →
     -- The equality argument builds in conversion.
-    Δ ⊢[l] A.subst (sbOfEnv ‖Δ‖ env) ≡ Aenv →
-    WfEnv Δ env Γ →
+    Δ ⊢[l] A.subst σ ≡ Aenv →
     (A, l) :: Γ ⊢[l'] B →
-    WfClosTp Δ l l' Aenv (.mk_tp Γ A env B)
+    ClosEqTp Δ l l' Aenv (.mk_tp Γ A env B) (B.subst <| Expr.up σ)
 
-/-- `WfClosTm Δ l l' A B b` -/
-inductive WfClosTm : Ctx → Nat → Nat → Expr → Expr → Clos → Prop
-  | clos_tm {Δ Γ A B Aenv Benv b env l l'} :
-    Δ ⊢[l] A.subst (sbOfEnv ‖Δ‖ env) ≡ Aenv →
-    (Aenv, l) :: Δ ⊢[l'] (B.subst <| Expr.up (sbOfEnv ‖Δ‖ env)) ≡ Benv →
-    WfEnv Δ env Γ →
+/-- `ClosEqTm Δ l l' A B vb b` -/
+inductive ClosEqTm : Ctx → Nat → Nat → Expr → Expr → Clos → Expr → Prop
+  | clos_tm {Δ Γ A B Aenv Benv b env σ l l'} :
+    EnvEqSb Δ env σ Γ →
+    Δ ⊢[l] A.subst σ ≡ Aenv →
+    (Aenv, l) :: Δ ⊢[l'] (B.subst <| Expr.up σ) ≡ Benv →
     (A, l) :: Γ ⊢[l'] b : B →
-    WfClosTm Δ l l' Aenv Benv (.mk_tm Γ A env b)
+    ClosEqTm Δ l l' Aenv Benv (.mk_tm Γ A env b) (b.subst <| Expr.up σ)
 
-inductive WfEnv : Ctx → List Val → Ctx → Prop
-  /- Possible optimization: allow `WfEnv Γ [] Γ`
+inductive EnvEqSb : Ctx → List Val → (Nat → Expr) → Ctx → Prop
+  /- Possible optimization: allow `EnvEqSb Γ [] Expr.bvar Γ`
   and replace `envOfLen ‖Γ‖` by `[]`. -/
-  | nil {Γ} : WfCtx Γ → WfEnv Γ [] []
-  | snoc {Δ Γ A v E l} :
-    WfEnv Δ E Γ →
+  | nil {Γ} (σ) : WfCtx Γ → EnvEqSb Γ [] σ []
+  | snoc {Δ Γ A vt t E σ l} :
+    EnvEqSb Δ E σ Γ →
     Γ ⊢[l] A →
-    WfValTm Δ l v (A.subst (sbOfEnv ‖Δ‖ E)) →
-    WfEnv Δ (v :: E) ((A, l) :: Γ)
+    ValEqTm Δ l vt t (A.subst σ) →
+    EnvEqSb Δ (vt :: E) (Expr.snoc σ t) ((A, l) :: Γ)
 end
 
 /-! ## Well-formed evaluation environments -/
 
-namespace WfEnv
+namespace EnvEqSb
 
-theorem wf_dom {Δ} : ∀ {E Γ}, WfEnv Δ E Γ → WfCtx Δ := by
-  mutual_induction WfEnv
+theorem wf_dom {Δ} : ∀ {E σ Γ}, EnvEqSb Δ E σ Γ → WfCtx Δ := by
+  mutual_induction EnvEqSb
   all_goals grind
 
-theorem wf_cod {Δ} : ∀ {E Γ}, WfEnv Δ E Γ → WfCtx Γ := by
-  mutual_induction WfEnv
+theorem wf_cod {Δ} : ∀ {E σ Γ}, EnvEqSb Δ E σ Γ → WfCtx Γ := by
+  mutual_induction EnvEqSb
   all_goals grind [WfCtx.nil, WfCtx.snoc]
 
-theorem eq_length {Δ} : ∀ {E Γ}, WfEnv Δ E Γ → ‖E‖ = ‖Γ‖ := by
-  mutual_induction WfEnv
+theorem eq_length {Δ} : ∀ {E σ Γ}, EnvEqSb Δ E σ Γ → ‖E‖ = ‖Γ‖ := by
+  mutual_induction EnvEqSb
   all_goals intros; try exact True.intro
   all_goals simp; try grind
 
-theorem lookup_lt {Δ Γ E i A l} : WfEnv Δ E Γ → Lookup Γ i A l → i < ‖E‖ :=
+theorem lookup_lt {Δ Γ E σ i A l} : EnvEqSb Δ E σ Γ → Lookup Γ i A l → i < ‖E‖ :=
   fun env lk => env.eq_length ▸ lk.lt_length
 
-theorem lookup_wf {Δ} : ∀ {E Γ}, (env : WfEnv Δ E Γ) →
+theorem lookup_eq {Δ} : ∀ {E σ Γ}, (env : EnvEqSb Δ E σ Γ) →
     ∀ {A i l}, (lk : Lookup Γ i A l) →
-    WfValTm Δ l (E[i]'(env.lookup_lt lk)) (A.subst (sbOfEnv ‖Δ‖ E)) := by
-  mutual_induction WfEnv
+    ValEqTm Δ l (E[i]'(env.lookup_lt lk)) (σ i) (A.subst σ) := by
+  mutual_induction EnvEqSb
   all_goals intros; try exact True.intro
   case nil lk => cases lk
   case snoc E A v ih _ _ _ _ lk =>
     rcases lk with _ | ⟨_, _, lk⟩
-    . convert v using 1
-      autosubst
-      rw [A.sbOfEnv_irrel (E.eq_length ▸ Nat.le_refl _)]
-    . convert ih lk using 1
-      autosubst
-      rw [A.wf_ctx.lookup_wf lk |>.sbOfEnv_irrel (E.eq_length ▸ Nat.le_refl _)]
+    . convert v using 1; autosubst
+    . convert ih lk using 1; autosubst
 
-theorem sbOfEnv_app {Δ Γ A E i l} (env : WfEnv Δ E Γ) (lk : Lookup Γ i A l) :
-    sbOfEnv ‖Δ‖ E 0 i = (E[i]'(env.lookup_lt lk)).toExpr ‖Δ‖ := by
-  simp [sbOfEnv, sbOfTms, List.getElem?_eq_some_iff.mpr ⟨env.lookup_lt lk, rfl⟩]
+lemma Expr.eq_snoc_self (σ : Nat → Expr) : σ = Expr.snoc (Expr.comp σ Expr.wk) (σ 0) := by
+  ext i; cases i <;> rfl
 
-theorem mk : ∀ {Γ}, WfCtx Γ → ∀ {Δ} {E : List Val}, WfCtx Δ → (eq : ‖Γ‖ = ‖E‖) →
+theorem mk : ∀ {Γ}, WfCtx Γ → ∀ {Δ} {E : List Val} {σ}, WfCtx Δ → (eq : ‖Γ‖ = ‖E‖) →
     (∀ {i A l}, (lk : Lookup Γ i A l) →
-      WfValTm Δ l (E[i]'(eq ▸ lk.lt_length)) (A.subst (sbOfEnv ‖Δ‖ E))) →
-    WfEnv Δ E Γ := by
+      ValEqTm Δ l (E[i]'(eq ▸ lk.lt_length)) (σ i) (A.subst σ)) →
+    EnvEqSb Δ E σ Γ := by
   mutual_induction WfCtx
   all_goals intros; try exact True.intro
   case nil eq _ =>
     have := List.length_eq_zero_iff.mp eq.symm
-    grind [WfEnv.nil]
-  case snoc A ih _ _ E Δ eq h =>
+    grind [EnvEqSb.nil]
+  case snoc ih _ _ E σ Δ eq h =>
     cases E
     . cases eq
     . replace eq := Nat.succ_inj.mp eq
-      apply WfEnv.snoc
+      rw [Expr.eq_snoc_self σ]
+      apply EnvEqSb.snoc
       . refine ih Δ eq fun lk => ?_
         convert h (lk.succ ..) using 1; autosubst
-        conv => rhs; rw [A.wf_ctx.lookup_wf lk |>.sbOfEnv_irrel <| eq ▸ Nat.le_refl _]
       . assumption
       . convert h (Lookup.zero ..) using 1; autosubst
-        conv => rhs; rw [A.sbOfEnv_irrel <| eq ▸ Nat.le_refl _]
 
-end WfEnv
+end EnvEqSb
 
 /-! ## Values are well-typed as expressions -/
 
-attribute [local grind] Val.toExpr Neut.toExpr Clos.toExpr in
-theorem wf_toExpr {Γ} :
-    (∀ {l A}, WfValTp Γ l A → Γ ⊢[l] A.toExpr ‖Γ‖) ∧
-    (∀ {l t A}, WfValTm Γ l t A → Γ ⊢[l] t.toExpr ‖Γ‖ : A) ∧
-    (∀ {l t A}, WfNeutTm Γ l t A → Γ ⊢[l] t.toExpr ‖Γ‖ : A) ∧
-    (∀ {l l' A B}, WfClosTp Γ l l' A B → (A, l) :: Γ ⊢[l'] B.toExpr ‖Γ‖) ∧
-    (∀ {l l' A B b}, WfClosTm Γ l l' A B b → (A, l) :: Γ ⊢[l'] b.toExpr ‖Γ‖ : B) ∧
-    (∀ {E Γ'}, WfEnv Γ E Γ' → ∀ (k), WfSb Γ (sbOfEnv ‖Γ‖ E k) Γ') := by
-  mutual_induction WfValTp
+theorem wf_expr {Γ} :
+    (∀ {l vA A}, ValEqTp Γ l vA A → Γ ⊢[l] A) ∧
+    (∀ {l vt t A}, ValEqTm Γ l vt t A → Γ ⊢[l] t : A) ∧
+    (∀ {l vt t A}, NeutEqTm Γ l vt t A → Γ ⊢[l] t : A) ∧
+    (∀ {l l' A vB B}, ClosEqTp Γ l l' A vB B → (A, l) :: Γ ⊢[l'] B) ∧
+    (∀ {l l' A B vb b}, ClosEqTm Γ l l' A B vb b → (A, l) :: Γ ⊢[l'] b : B) ∧
+    (∀ {E σ Γ'}, EnvEqSb Γ E σ Γ' → WfSb Γ σ Γ') := by
+  mutual_induction ValEqTp
   all_goals dsimp; intros
   case pi => grind [WfTp.pi]
   case sigma => grind [WfTp.sigma]
   case univ => grind [WfTp.univ]
   case el => grind [WfTp.el]
+  case conv_tp => grind [EqTp.wf_right]
   case lam => grind [WfTm.lam]
   case pair => grind [WfTm.pair]
   case code => grind [WfTm.code]
   case neut_tm => grind
-  case conv_nf => grind [WfTm.conv]
-  case bvar Γ lk =>
-    unfold Neut.toExpr
-    convert WfTm.bvar Γ lk using 2
-    have := lk.lt_length
-    omega
+  case conv_nf tt' AA' _ => exact tt'.wf_right.conv AA'
+  case bvar Γ lk => exact WfTm.bvar Γ lk
   case app => grind [WfTm.app]
   case fst => grind [WfTm.fst]
   case snd => grind [WfTm.snd]
-  case conv_neut => grind [WfTm.conv]
-  case clos_tp Aenv _ B sb =>
-    have := B.subst (sb 0 |>.up B.wf_ctx.inv_snoc)
-    have := this.conv_binder Aenv
-    convert this using 1
-    rw [Clos.toExpr]
-  case clos_tm Aenv Benv _ b env =>
-    unfold Clos.toExpr
-    have := b.subst (env 0 |>.up b.wf_ctx.inv_snoc)
+  case conv_neut nn' AA' _ => exact nn'.wf_right.conv AA'
+  case clos_tp Aenv B σ =>
+    have := B.subst (σ.up B.wf_binder)
+    exact this.conv_binder Aenv
+  case clos_tm Aenv Benv b σ =>
+    have := b.subst (σ.up b.wf_binder)
     have := this.conv_ctx (EqCtx.refl Aenv.wf_ctx |>.snoc Aenv)
     exact this.conv Benv
   case nil => apply WfSb.terminal; assumption
-  case snoc E A _ _ _ _ =>
-    rw [sbOfEnv_cons]
-    apply WfSb.snoc
-    . grind
-    . grind
-    . rw [A.sbOfEnv_irrel (E.eq_length ▸ Nat.le_refl _)]; grind
+  case snoc => grind [WfSb.snoc]
 
-theorem WfValTp.wf_toExpr {Γ l A} (h : WfValTp Γ l A) : Γ ⊢[l] A.toExpr ‖Γ‖ :=
-  _root_.wf_toExpr.1 h
+theorem ValEqTp.wf_tp {Γ l vA A} (h : ValEqTp Γ l vA A) : Γ ⊢[l] A :=
+  _root_.wf_expr.1 h
 
-theorem WfValTm.wf_toExpr {Γ l t A} (h : WfValTm Γ l t A) : Γ ⊢[l] t.toExpr ‖Γ‖ : A :=
-  _root_.wf_toExpr.2.1 h
+theorem ValEqTm.wf_tm {Γ l vt t A} (h : ValEqTm Γ l vt t A) : Γ ⊢[l] t : A :=
+  _root_.wf_expr.2.1 h
 
-theorem WfNeutTm.wf_toExpr {Γ l t A} (h : WfNeutTm Γ l t A) : Γ ⊢[l] t.toExpr ‖Γ‖ : A :=
-  _root_.wf_toExpr.2.2.1 h
+theorem NeutEqTm.wf_tm {Γ l vt t A} (h : NeutEqTm Γ l vt t A) : Γ ⊢[l] t : A :=
+  _root_.wf_expr.2.2.1 h
 
-theorem WfClosTp.wf_toExpr {Γ l l' A B} (h : WfClosTp Γ l l' A B) :
-    (A, l) :: Γ ⊢[l'] B.toExpr ‖Γ‖ :=
-  _root_.wf_toExpr.2.2.2.1 h
+theorem ClosEqTp.wf_tp {Γ l l' A vB B} (h : ClosEqTp Γ l l' A vB B) :
+    (A, l) :: Γ ⊢[l'] B :=
+  _root_.wf_expr.2.2.2.1 h
 
-theorem WfClosTm.wf_toExpr {Γ A B b l l'} (h : WfClosTm Γ l l' A B b) :
-    (A, l) :: Γ ⊢[l'] b.toExpr ‖Γ‖ : B :=
-  _root_.wf_toExpr.2.2.2.2.1 h
+theorem ClosEqTm.wf_tm {Γ l l' A B vb b} (h : ClosEqTm Γ l l' A B vb b) :
+    (A, l) :: Γ ⊢[l'] b : B :=
+  _root_.wf_expr.2.2.2.2.1 h
 
-theorem WfEnv.wf_sbOfEnv {Δ E Γ} (h : WfEnv Δ E Γ) : WfSb Δ (sbOfEnv ‖Δ‖ E) Γ :=
-  _root_.wf_toExpr.2.2.2.2.2 h 0
+theorem EnvEqSb.wf_sb {Δ E σ Γ} (h : EnvEqSb Δ E σ Γ) : WfSb Δ σ Γ :=
+  _root_.wf_expr.2.2.2.2.2 h
 
-/-! ## Values are closed under conversion -/
+theorem ValEqTm.conv_tp {Γ A A' vt t l} :
+    ValEqTm Γ l vt t A → Γ ⊢[l] A ≡ A' → ValEqTm Γ l vt t A' :=
+  fun h eq => h.conv_nf (EqTm.refl_tm h.wf_tm) eq
+
+theorem NeutEqTm.conv_tp {Γ A A' vt t l} :
+    NeutEqTm Γ l vt t A → Γ ⊢[l] A ≡ A' → NeutEqTm Γ l vt t A' :=
+  fun h eq => h.conv_neut (EqTm.refl_tm h.wf_tm) eq
+
+/-! ## Values are closed under context conversion -/
 
 attribute [local grind] EqCtx.length_eq in
 theorem conv_ctx {Γ} :
-    (∀ {l A}, WfValTp Γ l A → ∀ {Γ'}, EqCtx Γ Γ' → WfValTp Γ' l A) ∧
-    (∀ {l t A}, WfValTm Γ l t A → ∀ {Γ'}, EqCtx Γ Γ' → WfValTm Γ' l t A) ∧
-    (∀ {l t A}, WfNeutTm Γ l t A → ∀ {Γ'}, EqCtx Γ Γ' → WfNeutTm Γ' l t A) ∧
-    (∀ {l l' A B}, WfClosTp Γ l l' A B → ∀ {Γ'}, EqCtx Γ Γ' → WfClosTp Γ' l l' A B) ∧
-    (∀ {l l' A B b}, WfClosTm Γ l l' A B b → ∀ {Γ'}, EqCtx Γ Γ' → WfClosTm Γ' l l' A B b) ∧
-    (∀ {E Δ}, WfEnv Γ E Δ → ∀ {Γ'}, EqCtx Γ Γ' → WfEnv Γ' E Δ) := by
-  mutual_induction WfValTp
-  all_goals intros; try exact True.intro
-  case pi => grind [WfValTp.pi, EqTp.refl_tp]
-  case sigma => grind [WfValTp.sigma, EqTp.refl_tp]
-  case univ => grind [WfValTp.univ, EqCtx.wf_right]
-  case el => grind [WfValTp.el]
-  case lam eq => grind [WfValTm.lam]
+    (∀ {l vA A}, ValEqTp Γ l vA A → ∀ {Γ'}, EqCtx Γ Γ' → ValEqTp Γ' l vA A) ∧
+    (∀ {l vt t A}, ValEqTm Γ l vt t A → ∀ {Γ'}, EqCtx Γ Γ' → ValEqTm Γ' l vt t A) ∧
+    (∀ {l vt t A}, NeutEqTm Γ l vt t A → ∀ {Γ'}, EqCtx Γ Γ' → NeutEqTm Γ' l vt t A) ∧
+    (∀ {l l' A vB B}, ClosEqTp Γ l l' A vB B → ∀ {Γ'}, EqCtx Γ Γ' → ClosEqTp Γ' l l' A vB B) ∧
+    (∀ {l l' A B vb b}, ClosEqTm Γ l l' A B vb b → ∀ {Γ'}, EqCtx Γ Γ' →
+      ClosEqTm Γ' l l' A B vb b) ∧
+    (∀ {E σ Δ}, EnvEqSb Γ E σ Δ → ∀ {Γ'}, EqCtx Γ Γ' → EnvEqSb Γ' E σ Δ) := by
+  mutual_induction ValEqTp
+  all_goals intros
+  case pi => grind [ValEqTp.pi]
+  case sigma => grind [ValEqTp.sigma]
+  case univ => grind [ValEqTp.univ, EqCtx.wf_right]
+  case el => grind [ValEqTp.el]
+  case conv_tp => grind [ValEqTp.conv_tp, EqTp.conv_ctx]
+  case lam eq => grind [ValEqTm.lam]
   case pair B _ _ _ _ _ eq =>
-    apply WfValTm.pair (B.conv_ctx (eq.snoc <| EqTp.refl_tp B.wf_ctx.inv_snoc)) <;>
+    apply ValEqTm.pair (B.conv_ctx (eq.snoc <| EqTp.refl_tp B.wf_binder)) <;>
       grind
-  case code => grind [WfValTm.code]
-  case neut_tm => grind [WfValTm.neut_tm]
-  case conv_nf => grind [EqTp.conv_ctx, WfValTm.conv_nf]
+  case code => grind [ValEqTm.code]
+  case neut_tm => grind [ValEqTm.neut_tm]
+  case conv_nf => grind [EqTm.conv_ctx, EqTp.conv_ctx, ValEqTm.conv_nf]
   case bvar lk _ eq =>
     have ⟨A', _, lk'⟩ := Lookup.of_lt_length <| eq.length_eq ▸ lk.lt_length
     obtain ⟨rfl, eqA⟩ := eq.lookup_eq lk lk'
-    have := WfNeutTm.bvar eq.wf_right lk'
+    have := NeutEqTm.bvar eq.wf_right lk'
     rw [eq.length_eq]
-    exact WfNeutTm.conv_neut this (eqA.symm_tp.conv_ctx eq)
-  case app eq =>
-    rw [eq.length_eq]
-    grind [WfNeutTm.app]
-  case fst => grind [WfNeutTm.fst]
-  case snd B _ _ _ eq =>
-    rw [eq.length_eq]
-    grind [WfNeutTm.snd]
-  case conv_neut => grind [EqTp.conv_ctx, WfNeutTm.conv_neut]
-  case clos_tp Aeq env _ _ _ eq =>
-    rw [eq.length_eq] at Aeq
-    grind [WfClosTp.clos_tp, EqTp.conv_ctx]
-  case clos_tm Aeq Beq env b _ _ eq =>
-    rw [eq.length_eq] at Aeq Beq
-    apply WfClosTm.clos_tm _ (Beq.conv_ctx _)
-    all_goals grind [EqTp.conv_ctx, EqCtx.snoc, EqTp.refl_tp, EqTp.wf_right]
-  case nil eq => exact .nil eq.wf_right
-  case snoc => grind [WfEnv.snoc]
+    exact NeutEqTm.conv_neut this (EqTm.refl_tm (wf_expr.2.2.1 this)) (eqA.symm_tp.conv_ctx eq)
+  case app eq => grind [NeutEqTm.app]
+  case fst => grind [NeutEqTm.fst]
+  case snd => grind [NeutEqTm.snd]
+  case conv_neut => grind [EqTm.conv_ctx, EqTp.conv_ctx, NeutEqTm.conv_neut]
+  case clos_tp => grind [ClosEqTp.clos_tp, EqTp.conv_ctx]
+  case clos_tm Aeq Beq b env _ eq =>
+    exact ClosEqTm.clos_tm (env eq) (Aeq.conv_ctx eq)
+      (Beq.conv_ctx <| eq.snoc <| EqTp.refl_tp Aeq.wf_right)
+      (b.conv_ctx b.wf_ctx.eq_self)
+  case nil eq => exact .nil _ eq.wf_right
+  case snoc => grind [EnvEqSb.snoc]
 
-theorem WfValTp.conv_ctx {Γ Γ' l A} : WfValTp Γ l A → EqCtx Γ Γ' → WfValTp Γ' l A :=
+theorem ValEqTp.conv_ctx {Γ Γ' l vA A} : ValEqTp Γ l vA A → EqCtx Γ Γ' → ValEqTp Γ' l vA A :=
   fun h eq => _root_.conv_ctx.1 h eq
 
-theorem WfValTm.conv_ctx {Γ Γ' l t A} : WfValTm Γ l t A → EqCtx Γ Γ' → WfValTm Γ' l t A :=
+theorem ValEqTm.conv_ctx {Γ Γ' l vt t A} : ValEqTm Γ l vt t A → EqCtx Γ Γ' →
+    ValEqTm Γ' l vt t A :=
   fun h eq => _root_.conv_ctx.2.1 h eq
 
-theorem WfNeutTm.conv_ctx {Γ Γ' l t A} : WfNeutTm Γ l t A → EqCtx Γ Γ' → WfNeutTm Γ' l t A :=
+theorem NeutEqTm.conv_ctx {Γ Γ' l vt t A} : NeutEqTm Γ l vt t A → EqCtx Γ Γ' →
+    NeutEqTm Γ' l vt t A :=
   fun h eq => _root_.conv_ctx.2.2.1 h eq
 
-theorem WfClosTp.conv_ctx {Γ Γ' l l' A B} : WfClosTp Γ l l' A B → EqCtx Γ Γ' →
-    WfClosTp Γ' l l' A B :=
+theorem ClosEqTp.conv_ctx {Γ Γ' l l' A vB B} : ClosEqTp Γ l l' A vB B → EqCtx Γ Γ' →
+    ClosEqTp Γ' l l' A vB B :=
   fun h eq => _root_.conv_ctx.2.2.2.1 h eq
 
-theorem WfClosTm.conv_ctx {Γ Γ' l l' A B b} :
-    WfClosTm Γ l l' A B b → EqCtx Γ Γ' → WfClosTm Γ' l l' A B b :=
+theorem ClosEqTm.conv_ctx {Γ Γ' l l' A B vb b} :
+    ClosEqTm Γ l l' A B vb b → EqCtx Γ Γ' → ClosEqTm Γ' l l' A B vb b :=
   fun h eq => _root_.conv_ctx.2.2.2.2.1 h eq
 
-theorem WfEnv.conv_dom {Δ Δ' Γ E} : WfEnv Δ E Γ → EqCtx Δ Δ' → WfEnv Δ' E Γ :=
+theorem EnvEqSb.conv_dom {Δ Δ' E σ Γ} : EnvEqSb Δ E σ Γ → EqCtx Δ Δ' → EnvEqSb Δ' E σ Γ :=
   fun h eq => _root_.conv_ctx.2.2.2.2.2 h eq
 
 /-! ## Environments from contexts -/
@@ -481,81 +406,335 @@ theorem envOfLen_succ (n : Nat) : envOfLen (n + 1) = (.neut <| .bvar n) :: envOf
   dsimp
   omega
 
-@[autosubst]
-theorem sbOfEnv_envOfLen (n : Nat) : sbOfEnv n (envOfLen n) = Expr.bvar := by
-  ext i
-  simp [sbOfEnv, sbOfTms, envOfLen, Val.toExpr, Neut.toExpr]
-  split_ifs <;> simp
-  . omega
-
-theorem envOfLen_wf {Γ} : WfCtx Γ → WfEnv Γ (envOfLen ‖Γ‖) Γ := by
+theorem envOfLen_wf {Γ} : WfCtx Γ → EnvEqSb Γ (envOfLen ‖Γ‖) Expr.bvar Γ := by
   intro Γ
-  refine WfEnv.mk Γ Γ (length_envOfLen _).symm fun lk => ?_
-  conv => enter [3]; simp only [envOfLen, List.getElem_ofFn]
-  apply WfValTm.neut_tm
-  apply WfNeutTm.bvar Γ
-  convert lk; autosubst
+  refine EnvEqSb.mk Γ Γ (length_envOfLen _).symm fun lk => ?_
+  simp only [envOfLen, List.getElem_ofFn]
+  apply ValEqTm.neut_tm
+  apply NeutEqTm.bvar Γ
+  convert lk using 1; autosubst
 
-/-! ## Inversion for well-formed values -/
+/-! ## Weakening is free -/
 
-theorem WfValTp.inv_pi {Γ vA vB l k k'} : WfValTp Γ l (.pi k k' vA vB) →
-    l = max k k' ∧ WfValTp Γ k vA ∧ WfClosTp Γ k k' (vA.toExpr ‖Γ‖) vB := by
-  suffices ∀ {l t}, WfValTp Γ l t →
-      ∀ {vA vB k k'}, t = .pi k k' vA vB →
-        l = max k k' ∧ WfValTp Γ k vA ∧ WfClosTp Γ k k' (vA.toExpr ‖Γ‖) vB from
+theorem wk_all {Γ} :
+    (∀ {l vA A}, ValEqTp Γ l vA A → ∀ {C k}, Γ ⊢[k] C →
+      ValEqTp ((C,k) :: Γ) l vA (A.subst Expr.wk)) ∧
+    (∀ {l vt t A}, ValEqTm Γ l vt t A → ∀ {C k}, Γ ⊢[k] C →
+      ValEqTm ((C,k) :: Γ) l vt (t.subst Expr.wk) (A.subst Expr.wk)) ∧
+    (∀ {l vt t A}, NeutEqTm Γ l vt t A → ∀ {C k}, Γ ⊢[k] C →
+      NeutEqTm ((C,k) :: Γ) l vt (t.subst Expr.wk) (A.subst Expr.wk)) ∧
+    (∀ {l l' A vB B}, ClosEqTp Γ l l' A vB B → ∀ {C k}, Γ ⊢[k] C →
+      ClosEqTp ((C,k) :: Γ) l l' (A.subst Expr.wk) vB (B.subst (Expr.up Expr.wk))) ∧
+    (∀ {l l' A B vb b}, ClosEqTm Γ l l' A B vb b → ∀ {C k}, Γ ⊢[k] C →
+      ClosEqTm ((C,k) :: Γ) l l' (A.subst Expr.wk) (B.subst (Expr.up Expr.wk))
+        vb (b.subst (Expr.up Expr.wk))) ∧
+    (∀ {E σ Δ}, EnvEqSb Γ E σ Δ → ∀ {C k}, Γ ⊢[k] C →
+      EnvEqSb ((C,k) :: Γ) E (Expr.comp Expr.wk σ) Δ) := by
+  mutual_induction ValEqTp
+  all_goals intros; try dsimp [Expr.subst] at *
+  case pi => grind [ValEqTp.pi]
+  case sigma => grind [ValEqTp.sigma]
+  case univ => grind [ValEqTp.univ, WfCtx.snoc]
+  case el => grind [ValEqTp.el]
+  case conv_tp => grind [ValEqTp.conv_tp, EqTp.subst, WfSb.wk]
+  case lam eq => grind [ValEqTm.lam]
+  case pair B _ _ iht ihu _ _ C =>
+    have := B.subst (WfSb.wk C |>.up B.wf_binder)
+    apply ValEqTm.pair this (iht C) (by convert ihu C using 1; autosubst)
+  case code => grind [ValEqTm.code]
+  case neut_tm => grind [ValEqTm.neut_tm]
+  case conv_nf => grind [ValEqTm.conv_nf, EqTp.subst, EqTm.subst, WfSb.wk]
+  case bvar Γ lk _ _ C =>
+    convert NeutEqTm.bvar (Γ.snoc C) (.succ _ _ lk) using 1; grind
+  case app ihf iha _ _ C =>
+    convert NeutEqTm.app (ihf C) (iha C) using 1; autosubst
+  case fst => grind [NeutEqTm.fst]
+  case snd ih _ _ C =>
+    convert NeutEqTm.snd (ih C) using 1; autosubst
+  case conv_neut => grind [NeutEqTm.conv_neut, EqTp.subst, EqTm.subst, WfSb.wk]
+  case clos_tp Aeq B ih _ _ C =>
+    have := Aeq.subst (WfSb.wk C)
+    convert ClosEqTp.clos_tp (ih C) (by convert this using 1; autosubst) B using 1
+    autosubst
+  case clos_tm Aeq Beq b ih _ _ C =>
+    have CAeq := Aeq.subst <| WfSb.wk C
+    have CBeq := Beq.subst <| (WfSb.wk C).up Aeq.wf_right
+    have := ClosEqTm.clos_tm (ih C)
+      (by convert CAeq using 1; autosubst)
+      (by convert CBeq using 1; autosubst)
+      b
+    convert this using 1; autosubst
+  case nil C => apply EnvEqSb.nil _ (C.wf_ctx.snoc C)
+  case snoc =>
+    simp only [autosubst] at *
+    grind [EnvEqSb.snoc]
+
+/-! ## Inversion for value relations -/
+
+theorem ValEqTp.inv_pi {Γ C vA vB l k k'} : ValEqTp Γ l (.pi k k' vA vB) C →
+    l = max k k' ∧ ∃ A B, ValEqTp Γ k vA A ∧ ClosEqTp Γ k k' A vB B ∧
+      (Γ ⊢[max k k'] C ≡ .pi k k' A B) := by
+  suffices ∀ {l vC C}, ValEqTp Γ l vC C →
+      ∀ {vA vB k k'}, vC = .pi k k' vA vB →
+        l = max k k' ∧ ∃ A B, ValEqTp Γ k vA A ∧ ClosEqTp Γ k k' A vB B ∧
+        (Γ ⊢[max k k'] C ≡ .pi k k' A B) from
     fun h => this h rfl
-  mutual_induction WfValTp
-  all_goals grind
+  mutual_induction ValEqTp
+  all_goals grind [WfTp.pi, ClosEqTp.wf_tp]
 
-theorem WfValTp.inv_sigma {Γ vA vB l k k'} : WfValTp Γ l (.sigma k k' vA vB) →
-    l = max k k' ∧ WfValTp Γ k vA ∧ WfClosTp Γ k k' (vA.toExpr ‖Γ‖) vB := by
-  suffices ∀ {l t}, WfValTp Γ l t →
-      ∀ {vA vB k k'}, t = .sigma k k' vA vB →
-        l = max k k' ∧ WfValTp Γ k vA ∧ WfClosTp Γ k k' (vA.toExpr ‖Γ‖) vB from
+theorem ValEqTp.inv_sigma {Γ C vA vB l k k'} : ValEqTp Γ l (.sigma k k' vA vB) C →
+    l = max k k' ∧ ∃ A B, ValEqTp Γ k vA A ∧ ClosEqTp Γ k k' A vB B ∧
+      (Γ ⊢[max k k'] C ≡ .sigma k k' A B) := by
+  suffices ∀ {l vC C}, ValEqTp Γ l vC C →
+      ∀ {vA vB k k'}, vC = .sigma k k' vA vB →
+        l = max k k' ∧ ∃ A B, ValEqTp Γ k vA A ∧ ClosEqTp Γ k k' A vB B ∧
+        (Γ ⊢[max k k'] C ≡ .sigma k k' A B) from
     fun h => this h rfl
-  mutual_induction WfValTp
-  all_goals grind
+  mutual_induction ValEqTp
+  all_goals grind [WfTp.sigma, ClosEqTp.wf_tp]
 
-theorem WfValTm.inv_lam {Γ A C b l₀ l l'} : WfValTm Γ l₀ (.lam l l' A b) C →
-    l₀ = max l l' ∧ ∃ B, (WfClosTm Γ l l' A B b) ∧ (Γ ⊢[max l l'] C ≡ .pi l l' A B) := by
+theorem ValEqTp.inv_univ {Γ l k t} : ValEqTp Γ l (.univ k) t → l = k + 1 ∧
+    (Γ ⊢[k + 1] t ≡ .univ k) := by
+  suffices ∀ {l vt t}, ValEqTp Γ l vt t → ∀ {k}, vt = .univ k → l = k + 1 ∧
+      (Γ ⊢[k + 1] t ≡ .univ k) from
+    fun h => this h rfl
+  mutual_induction ValEqTp
+  all_goals grind [WfTp.univ]
+
+theorem ValEqTp.inv_el {Γ l va A} : ValEqTp Γ l (.el va) A →
+    ∃ a, ValEqTm Γ (l + 1) va a (.univ l) ∧ (Γ ⊢[l] A ≡ .el a) := by
+  suffices ∀ {l vA A}, ValEqTp Γ l vA A → ∀ {va}, vA = .el va →
+      ∃ a, ValEqTm Γ (l + 1) va a (.univ l) ∧ (Γ ⊢[l] A ≡ .el a) from
+    fun h => this h rfl
+  mutual_induction ValEqTp
+  all_goals grind [WfTp.el, ValEqTm.wf_tm]
+
+theorem ValEqTm.inv_lam {Γ C vb t l₀ l l'} : ValEqTm Γ l₀ (.lam l l' vb) t C →
+    l₀ = max l l' ∧ ∃ A B b, (ClosEqTm Γ l l' A B vb b) ∧
+      (Γ ⊢[max l l'] t ≡ .lam l l' A b : C) ∧
+      (Γ ⊢[max l l'] C ≡ .pi l l' A B) := by
   suffices
-      ∀ {l₀ t C}, WfValTm Γ l₀ t C → ∀ {A b l l'}, t = .lam l l' A b →
-        l₀ = max l l' ∧ ∃ B, (WfClosTm Γ l l' A B b) ∧ (Γ ⊢[max l l'] C ≡ .pi l l' A B) from
+      ∀ {l₀ vt t C}, ValEqTm Γ l₀ vt t C → ∀ {l l'}, vt = .lam l l' vb →
+        l₀ = max l l' ∧ ∃ A B b, (ClosEqTm Γ l l' A B vb b) ∧
+          (Γ ⊢[max l l'] t ≡ .lam l l' A b : C) ∧
+          (Γ ⊢[max l l'] C ≡ .pi l l' A B) from
     fun h => this h rfl
-  mutual_induction WfValTm
+  mutual_induction ValEqTm
   all_goals intros; try exact True.intro
   all_goals rename_i eq; cases eq
-  case lam b _ =>
-    refine ⟨rfl, _, by assumption, ?_⟩
-    rcases b with ⟨_, eq, _, _⟩
-    exact EqTp.refl_tp <| WfTp.pi eq.wf_right
-  case conv_nf =>
-    grind [EqTp.symm_tp, EqTp.trans_tp]
+  case conv_nf => grind [EqTm.conv_eq]
+  case lam => grind [WfTm.lam, ClosEqTm.wf_tm, WfTm.wf_tp, WfTp.pi]
 
-theorem WfValTm.inv_pair {Γ B C t u l₀ l l'} : WfValTm Γ l₀ (.pair l l' B t u) C →
-    l₀ = max l l' ∧ ∃ A, (WfValTm Γ l t A) ∧ (WfValTm Γ l' u (B.subst (t.toExpr ‖Γ‖).toSb)) ∧
+theorem ValEqTm.inv_pair {Γ C vt vu p l₀ l l'} : ValEqTm Γ l₀ (.pair l l' vt vu) p C →
+    l₀ = max l l' ∧ ∃ A B t u, (ValEqTm Γ l vt t A) ∧ (ValEqTm Γ l' vu u (B.subst t.toSb)) ∧
+      (Γ ⊢[max l l'] p ≡ .pair l l' B t u : C) ∧
       (Γ ⊢[max l l'] C ≡ .sigma l l' A B) := by
   suffices
-      ∀ {l₀ t₀ C}, WfValTm Γ l₀ t₀ C → ∀ {B t u l l'}, t₀ = .pair l l' B t u →
-        l₀ = max l l' ∧ ∃ A,
-          (WfValTm Γ l t A) ∧
-          (WfValTm Γ l' u (B.subst (t.toExpr ‖Γ‖).toSb)) ∧
+      ∀ {l₀ vp p C}, ValEqTm Γ l₀ vp p C → ∀ {vt vu l l'}, vp = .pair l l' vt vu →
+        l₀ = max l l' ∧ ∃ A B t u,
+          (ValEqTm Γ l vt t A) ∧
+          (ValEqTm Γ l' vu u (B.subst t.toSb)) ∧
+          (Γ ⊢[max l l'] p ≡ .pair l l' B t u : C) ∧
           (Γ ⊢[max l l'] C ≡ .sigma l l' A B) from
     fun h => this h rfl
-  mutual_induction WfValTm
+  mutual_induction ValEqTm
   all_goals intros; try exact True.intro
   all_goals rename_i eq; cases eq
-  case pair =>
-    refine ⟨rfl, _, by assumption, by assumption, ?_⟩
-    grind [EqTp.refl_tp, WfTp.sigma, WfClosTp.wf_toExpr]
-  case conv_nf =>
-    grind [EqTp.symm_tp, EqTp.trans_tp]
+  case conv_nf => grind [EqTm.conv_eq]
+  case pair => grind [WfTm.pair, ValEqTm.wf_tm, WfTp.sigma]
 
-theorem WfValTm.inv_neut {Γ A t l} : WfValTm Γ l (.neut t) A → WfNeutTm Γ l t A := by
-  suffices ∀ {l t A}, WfValTm Γ l t A → ∀ {n}, t = .neut n → (WfNeutTm Γ l n A) from
+theorem ValEqTm.inv_code {Γ C vA c l₀} : ValEqTm Γ l₀ (.code vA) c C →
+    ∃ l A, l₀ = l + 1 ∧ (ValEqTp Γ l vA A) ∧ (Γ ⊢[l₀] c ≡ .code A : C) ∧ (Γ ⊢[l₀] C ≡ .univ l) := by
+  suffices
+      ∀ {l₀ vc c C}, ValEqTm Γ l₀ vc c C → ∀ {vA}, vc = .code vA →
+        ∃ l A, l₀ = l + 1 ∧ (ValEqTp Γ l vA A) ∧ (Γ ⊢[l₀] c ≡ .code A : C) ∧ (Γ ⊢[l₀] C ≡ .univ l) from
     fun h => this h rfl
-  mutual_induction WfValTm
+  mutual_induction ValEqTm
   all_goals intros; try exact True.intro
   all_goals rename_i eq; cases eq
-  case neut_tm => assumption
-  case conv_nf eq _ _ ih => exact ih rfl |>.conv_neut eq
+  case conv_nf => grind [EqTm.conv_eq]
+  case code => grind [WfTp.univ, WfTm.code, ValEqTp.wf_tp, WfTp.wf_ctx]
+
+theorem ValEqTm.inv_neut {Γ A vt t l} : ValEqTm Γ l (.neut vt) t A → NeutEqTm Γ l vt t A := by
+  suffices ∀ {l vt t A}, ValEqTm Γ l vt t A → ∀ {n}, vt = .neut n → (NeutEqTm Γ l n t A) from
+    fun h => this h rfl
+  mutual_induction ValEqTm
+  all_goals grind [NeutEqTm.conv_neut]
+
+theorem NeutEqTm.inv_bvar {Γ A t i l} : NeutEqTm Γ l (.bvar i) t A →
+    ∃ A', Lookup Γ (‖Γ‖ - i - 1) A' l ∧
+      (Γ ⊢[l] t ≡ .bvar (‖Γ‖ - i - 1) : A) ∧ (Γ ⊢[l] A ≡ A') := by
+  suffices ∀ {l vn n A}, NeutEqTm Γ l vn n A → ∀ {i}, vn = .bvar i →
+      ∃ A', Lookup Γ (‖Γ‖ - i - 1) A' l ∧
+        (Γ ⊢[l] n ≡ .bvar (‖Γ‖ - i - 1) : A) ∧ (Γ ⊢[l] A ≡ A') from
+    fun h => this h rfl
+  mutual_induction NeutEqTm
+  all_goals intros; try exact True.intro
+  all_goals rename_i eq; cases eq
+  case bvar i _ Γwf lk =>
+    have := lk.lt_length
+    rw [show ‖Γ‖ - (‖Γ‖ - i - 1) - 1 = i by omega]
+    exact ⟨_, lk, EqTm.refl_tm (WfTm.bvar (by omega) lk), EqTp.refl_tp (Γwf.lookup_wf lk)⟩
+  case conv_neut => grind [EqTm.conv_eq]
+
+theorem NeutEqTm.inv_app {Γ C vf va t l₀ l l'} : NeutEqTm Γ l₀ (.app l l' vf va) t C →
+    l₀ = l' ∧ ∃ A B f a, NeutEqTm Γ (max l l') vf f (.pi l l' A B) ∧ ValEqTm Γ l va a A ∧
+      (Γ ⊢[l'] t ≡ .app l l' B f a : C) ∧ (Γ ⊢[l'] C ≡ B.subst a.toSb) := by
+  suffices ∀ {l₀ vn n C}, NeutEqTm Γ l₀ vn n C → ∀ {vf va l l'}, vn = .app l l' vf va →
+      l₀ = l' ∧ ∃ A B f a, NeutEqTm Γ (max l l') vf f (.pi l l' A B) ∧ ValEqTm Γ l va a A ∧
+        (Γ ⊢[l'] n ≡ .app l l' B f a : C) ∧ (Γ ⊢[l'] C ≡ B.subst a.toSb) from
+    fun h => this h rfl
+  mutual_induction NeutEqTm
+  all_goals intros; try exact True.intro
+  all_goals rename_i eq; cases eq
+  case conv_neut => grind [EqTm.conv_eq]
+  case app =>
+    grind [WfTm.app, ValEqTm.wf_tm, NeutEqTm.wf_tm, WfSb.toSb, WfTp.subst, WfTp.inv_pi, WfTm.wf_tp]
+
+theorem NeutEqTm.inv_fst {Γ C vp f l₀ l l'} : NeutEqTm Γ l₀ (.fst l l' vp) f C →
+    l₀ = l ∧ ∃ A B p, NeutEqTm Γ (max l l') vp p (.sigma l l' A B) ∧
+      (Γ ⊢[l] f ≡ .fst l l' A B p : C) ∧ (Γ ⊢[l] C ≡ A) := by
+  suffices ∀ {l₀ vn n C}, NeutEqTm Γ l₀ vn n C → ∀ {vp l l'}, vn = .fst l l' vp →
+      l₀ = l ∧ ∃ A B p, NeutEqTm Γ (max l l') vp p (.sigma l l' A B) ∧
+      (Γ ⊢[l] n ≡ .fst l l' A B p : C) ∧ (Γ ⊢[l] C ≡ A) from
+    fun h => this h rfl
+  mutual_induction NeutEqTm
+  all_goals intros; try exact True.intro
+  all_goals rename_i eq; cases eq
+  case conv_neut => grind [EqTm.conv_eq]
+  case fst =>
+    grind [WfTm.fst, NeutEqTm.wf_tm, WfTm.wf_tp, WfTp.inv_sigma, WfTp.wf_ctx, WfCtx.inv_snoc]
+
+theorem NeutEqTm.inv_snd {Γ C vp s l₀ l l'} : NeutEqTm Γ l₀ (.snd l l' vp) s C →
+    l₀ = l' ∧ ∃ A B p, NeutEqTm Γ (max l l') vp p (.sigma l l' A B) ∧
+      (Γ ⊢[l'] s ≡ .snd l l' A B p : C) ∧ (Γ ⊢[l'] C ≡ B.subst (Expr.fst l l' A B p).toSb) := by
+  suffices ∀ {l₀ vn n C}, NeutEqTm Γ l₀ vn n C → ∀ {vp l l'}, vn = .snd l l' vp →
+      l₀ = l' ∧ ∃ A B p, NeutEqTm Γ (max l l') vp p (.sigma l l' A B) ∧
+      (Γ ⊢[l'] n ≡ .snd l l' A B p : C) ∧ (Γ ⊢[l'] C ≡ B.subst (Expr.fst l l' A B p).toSb) from
+    fun h => this h rfl
+  mutual_induction NeutEqTm
+  all_goals intros; try exact True.intro
+  all_goals rename_i eq; cases eq
+  case conv_neut => grind [EqTm.conv_eq]
+  case snd =>
+    grind [WfTm.snd, NeutEqTm.wf_tm, WfTm.wf_tp, WfTp.inv_sigma, WfTp.wf_ctx, WfCtx.inv_snoc]
+
+/-! ## Functionality of value relations -/
+
+theorem uniq_all {Γ} :
+    (∀ {l vA A}, ValEqTp Γ l vA A → ∀ {A'}, ValEqTp Γ l vA A' → Γ ⊢[l] A ≡ A') ∧
+    (∀ {l vt t A}, ValEqTm Γ l vt t A → ∀ {t'}, ValEqTm Γ l vt t' A → Γ ⊢[l] t ≡ t' : A) ∧
+    /- Technicality: `ValEqTm` does not need the generalization to `A'`
+    because the only terms that 'forget' type information
+    are elimination forms which must be neutral as values. -/
+    (∀ {l vt t A}, NeutEqTm Γ l vt t A → ∀ {t' A'}, NeutEqTm Γ l vt t' A' →
+      (Γ ⊢[l] A ≡ A') ∧ (Γ ⊢[l] t ≡ t' : A)) ∧
+    (∀ {l l' A vB B}, ClosEqTp Γ l l' A vB B → ∀ {B'}, ClosEqTp Γ l l' A vB B' →
+      (A, l) :: Γ ⊢[l'] B ≡ B') ∧
+    (∀ {l l' A B vb b}, ClosEqTm Γ l l' A B vb b → ∀ {b'}, ClosEqTm Γ l l' A B vb b' →
+      (A, l) :: Γ ⊢[l'] b ≡ b' : B) ∧
+    (∀ {E σ Γ'}, EnvEqSb Γ E σ Γ' → ∀ {σ'}, EnvEqSb Γ E σ' Γ' →
+      EqSb Γ σ σ' Γ') := by
+  /- 2025-07-20: I think this could go by induction on `Val`,
+  but my `mutual_induction` tactic doesn't support that. -/
+  mutual_induction ValEqTp
+  all_goals dsimp; intros; try exact True.intro
+  case pi => grind [ValEqTp.inv_pi, cases ClosEqTp, ClosEqTp.clos_tp, EqTp.cong_pi]
+  case sigma => grind [ValEqTp.inv_sigma, cases ClosEqTp, ClosEqTp.clos_tp, EqTp.cong_sigma]
+  case univ h =>
+    have := h.inv_univ
+    grind
+  case el => grind [ValEqTp.inv_el, EqTp.cong_el]
+  case conv_tp => grind
+  case lam ihb _ vl =>
+    have ⟨_, _, _, _, vb, eqt, eq⟩ := vl.inv_lam
+    apply EqTm.trans_tm _ eqt.symm_tm
+    have ⟨_, _, _, Aeq, Beq⟩ := eq.inv_pi
+    gcongr
+    rcases vb with ⟨env, Aeq', Beq', b⟩
+    have Aeq'' := Aeq'.trans_tp Aeq.symm_tp
+    have := Beq'.conv_binder Aeq.symm_tp |>.trans_tp Beq.symm_tp
+    exact ihb ⟨env, Aeq'', this, b⟩
+  case pair iht ihu _ vp =>
+    have ⟨_, _, _, _, _, vt, vu, eqt, eq⟩ := vp.inv_pair
+    apply EqTm.trans_tm _ eqt.symm_tm
+    have ⟨_, _, _, Aeq, Beq⟩ := eq.inv_sigma
+    have := iht (vt.conv_tp Aeq.symm_tp)
+    gcongr
+    . apply ihu (vu.conv_tp _)
+      exact Beq.symm_tp.subst_eq (EqSb.toSb this.symm_tm)
+  case code => grind [ValEqTm.inv_code, EqTm.cong_code]
+  case neut_tm vn =>
+    have := vn.inv_neut
+    grind
+  case conv_nf Aeq ih _ vt =>
+    have := ih (vt.conv_tp Aeq.symm_tp)
+    grind [EqTm.conv_eq]
+  case bvar lk _ _ _ =>
+    have := lk.lt_length
+    grind [EqTm.conv_eq, Lookup.tp_uniq, NeutEqTm.inv_bvar]
+  case app ihf iha _ _ vn =>
+    have ⟨_, _, _, _, _, vf, va, eqt, eq⟩ := vn.inv_app
+    have ⟨peq, feq⟩ := ihf vf
+    have ⟨_, _, _, Aeq, Beq⟩ := peq.inv_pi
+    have aeq := iha <| va.conv_tp Aeq.symm_tp
+    refine ⟨?teq, (fun teq => ?_) ?teq⟩
+    . apply EqTp.trans_tp _ eq.symm_tp
+      exact Beq.subst_eq (EqSb.toSb aeq)
+    . apply EqTm.trans_tm _ <| eqt.symm_tm.conv_eq (by grind)
+      gcongr
+  case fst ih _ _ vn =>
+    have ⟨_, _, _, _, vp, eqt, eq⟩ := vn.inv_fst
+    have ⟨seq, peq⟩ := ih vp
+    have ⟨_, _, _, Aeq, Beq⟩ := seq.inv_sigma
+    constructor
+    . grind
+    . apply EqTm.trans_tm _ <| eqt.symm_tm.conv_eq (by grind)
+      gcongr
+  case snd ih _ _ vn =>
+    have ⟨_, _, _, _, vp, eqt, eq⟩ := vn.inv_snd
+    have ⟨seq, peq⟩ := ih vp
+    have ⟨_, _, _, Aeq, Beq⟩ := seq.inv_sigma
+    refine ⟨?teq2, (fun teq => ?_) ?teq2⟩
+    . apply EqTp.trans_tp _ eq.symm_tp
+      gcongr
+      apply EqSb.toSb
+      gcongr
+    . apply EqTm.trans_tm _ <| eqt.symm_tm.conv_eq (by grind)
+      gcongr
+  case conv_neut => grind [EqTm.conv_eq]
+  case clos_tp ih _ c =>
+    rcases c with ⟨env, Aeq, B⟩
+    have A := B.wf_binder
+    have := B.subst_eq ((ih env).up A)
+    exact this.conv_binder <| (A.subst_eq (ih env)).trans_tp Aeq
+  case clos_tm ih _ c =>
+    rcases c with ⟨env, Aeq, Beq, b⟩
+    have A := b.wf_binder
+    have := b.subst_eq ((ih env).symm.up A) |>.conv_binder Aeq
+      |>.conv_eq Beq
+    exact this.symm_tm
+  case nil => grind [EqSb.terminal]
+  case snoc => grind [cases EnvEqSb, EqSb.snoc, ValEqTm.conv_tp, WfTp.subst_eq]
+
+theorem ValEqTp.tp_uniq {Γ l vA A A'} : ValEqTp Γ l vA A → ValEqTp Γ l vA A' → Γ ⊢[l] A ≡ A' :=
+  fun h h' => uniq_all.1 h h'
+
+theorem ValEqTm.tm_uniq {Γ l vt t t' A} : ValEqTm Γ l vt t A → ValEqTm Γ l vt t' A →
+    Γ ⊢[l] t ≡ t' : A :=
+  fun h h' => uniq_all.2.1 h h'
+
+theorem NeutEqTm.tm_uniq {Γ l vn n A n' A'} : NeutEqTm Γ l vn n A → NeutEqTm Γ l vn n' A' →
+    Γ ⊢[l] n ≡ n' : A :=
+  fun h h' => uniq_all.2.2.1 h h' |>.2
+
+theorem ClosEqTp.tp_uniq {Γ l l' A vB B B'} : ClosEqTp Γ l l' A vB B → ClosEqTp Γ l l' A vB B' →
+    (A, l) :: Γ ⊢[l'] B ≡ B' :=
+  fun h h' => uniq_all.2.2.2.1 h h'
+
+theorem ClosEqTm.tm_uniq {Γ l l' A B vb b b'} : ClosEqTm Γ l l' A B vb b →
+    ClosEqTm Γ l l' A B vb b' → (A, l) :: Γ ⊢[l'] b ≡ b' : B :=
+  fun h h' => uniq_all.2.2.2.2.1 h h'
+
+theorem EnvEqSb.sb_uniq {Δ E σ σ' Γ} : EnvEqSb Δ E σ Γ → EnvEqSb Δ E σ' Γ → EqSb Δ σ σ' Γ :=
+  fun h h' => uniq_all.2.2.2.2.2 h h'
