GroupoidModel/Syntax/Typechecker/Evaluate.lean
@@ -3,7 +3,7 @@ import Qq
 import GroupoidModel.Syntax.GCongr
 import GroupoidModel.Syntax.Synth
 import GroupoidModel.Syntax.Injectivity
-import GroupoidModel.Syntax.Typechecker.Value
+import GroupoidModel.Syntax.Typechecker.ValueButItsARelationAndAnnotationsGone
 
 /-- Shorthand for `List.length` which is used a lot in this file. -/
 local notation "‖" l "‖" => List.length l
@@ -11,7 +11,7 @@ local notation "‖" l "‖" => List.length l
 -- /-- Hacks to use during development:
 -- `as_aux_lemma` blocks are not elaborated and kernel typechecking is off,
 -- speeding up interactive feedback. -/
--- FIXME: make `as_aux_lemma` or general `by` elaboration async for lower interaction latency.
+-- -- FIXME: make `as_aux_lemma` or general `by` elaboration async for lower interaction latency.
 -- macro_rules
 --   | `(tactic| as_aux_lemma => $s:tacticSeq) => `(tactic| sorry)
 -- set_option linter.unusedTactic false
@@ -28,392 +28,343 @@ mutual
 Note: Inferring implicits from `Q(...)` is pretty flaky,
 so all the arguments are explicit.
 
-Note: returning `Q(⋯ ∧ ⋯)` rather than `Q(⋯) × Q(⋯)`
-makes it easier to reuse proofs between the postconditions.
-
 Note: we use `as_aux_lemma` pervasively to minimize the size of produced proof terms. -/
 -- FIXME: by using `synthLvl`, we could also get rid of the `l` args in `eval*`.
-partial def evalTp (Δ : Ctx) (env : List Val) (Γ : Ctx) (l : Nat) (T : Expr)
-    (Δenv : Q(WfEnv $Δ $env $Γ))
+partial def evalTp (Δ : Q(Ctx)) (env : Q(List Val)) (σ : Q(Nat → Expr)) (Γ : Q(Ctx))
+    (l : Q(Nat)) (T : Q(Expr))
+    (Δenv : Q(EnvEqSb $Δ $env $σ $Γ))
     (ΓT : Q($Γ ⊢[$l] ($T))) :
-    Except String ((v : Val) ×
-      Q(WfValTp $Δ $l $v ∧
-        ($Δ ⊢[$l] ($v).toExpr ‖$Δ‖ ≡ ($T).subst (sbOfEnv ‖$Δ‖ $env)))) :=
+    Lean.MetaM ((v : Q(Val)) × Q(ValEqTp $Δ $l $v <| ($T).subst $σ)) :=
   match T with
-  | .pi l l' A B => do
-    let ⟨vA, vApfs⟩ ← evalTp Δ env Γ l A q($Δenv) q(($ΓT).inv_pi.2.wf_ctx.inv_snoc)
-    return ⟨.pi l l' vA (.mk_tp Γ A env B),
+  | ~q(.pi $l $l' $A $B) => do
+    let ⟨vA, vAeq⟩ ← evalTp Δ env σ Γ l A
+      q($Δenv)
+      q(by as_aux_lemma => exact ($ΓT).inv_pi.2.wf_binder)
+    return ⟨q(.pi $l $l' $vA (.mk_tp $Γ $A $env $B)),
       q(by as_aux_lemma =>
-        have ⟨vAwf, vAeq⟩ := $vApfs
+        simp +zetaDelta only [Expr.subst]
         obtain ⟨rfl, B⟩ := ($ΓT).inv_pi
-        constructor
-        . apply WfValTp.pi vAwf
-          exact WfClosTp.clos_tp vAeq.symm_tp $Δenv B
-        . simp only [Val.toExpr, Clos.toExpr, Expr.subst]
-          gcongr
-          exact B.subst (WfSb.up ($Δenv).wf_sbOfEnv B.wf_ctx.inv_snoc) |>.conv_ctx
-            (EqCtx.refl vAeq.wf_ctx |>.snoc vAeq.symm_tp)
+        apply ValEqTp.pi $vAeq
+        apply ClosEqTp.clos_tp $Δenv (EqTp.refl_tp ($vAeq).wf_tp) B
       )⟩
-  | .sigma l l' A B => do
-    let ⟨vA, vApfs⟩ ← evalTp Δ env Γ l A q($Δenv) q(($ΓT).inv_sigma.2.wf_ctx.inv_snoc)
-    return ⟨.sigma l l' vA (.mk_tp Γ A env B),
+  | ~q(.sigma $l $l' $A $B) => do
+    let ⟨vA, vAeq⟩ ← evalTp Δ env σ Γ l A
+      q($Δenv)
+      q(by as_aux_lemma => exact ($ΓT).inv_sigma.2.wf_binder)
+    return ⟨q(.sigma $l $l' $vA (.mk_tp $Γ $A $env $B)),
       q(by as_aux_lemma =>
-        have ⟨vAwf, vAeq⟩ := $vApfs
+        simp +zetaDelta only [Expr.subst]
         obtain ⟨rfl, B⟩ := ($ΓT).inv_sigma
-        constructor
-        . apply WfValTp.sigma vAwf
-          exact WfClosTp.clos_tp vAeq.symm_tp $Δenv B
-        . simp only [Val.toExpr, Clos.toExpr, Expr.subst]
-          gcongr
-          exact B.subst (WfSb.up ($Δenv).wf_sbOfEnv B.wf_ctx.inv_snoc) |>.conv_ctx
-            (EqCtx.refl vAeq.wf_ctx |>.snoc vAeq.symm_tp)
+        apply ValEqTp.sigma $vAeq
+        apply ClosEqTp.clos_tp $Δenv (EqTp.refl_tp ($vAeq).wf_tp) B
       )⟩
-  | .el a => do
-    let ⟨va, vapfs⟩ ← evalTm Δ env Γ (l + 1) a q($Δenv) q(($ΓT).inv_el.with_synthTp)
-    return ⟨.el va,
+  | ~q(.el $a) => do
+    let ⟨va, vaeq⟩ ← evalTm Δ env σ Γ q($l + 1) a
+      q($Δenv)
+      q(by as_aux_lemma => exact ($ΓT).inv_el.with_synthTp)
+    return ⟨q(.el $va),
       q(by as_aux_lemma =>
-        have ⟨vawf, vaeq⟩ := $vapfs
-        have := ($ΓT).inv_el.tp_eq_synthTp.symm_tp.subst ($Δenv).wf_sbOfEnv
-        simp only [Expr.subst, Val.toExpr] at this ⊢
-        exact ⟨WfValTp.el <| vawf.conv_nf this, EqTp.cong_el <| vaeq.conv_eq this⟩
+        simp +zetaDelta only [Expr.subst]
+        apply ValEqTp.el <| ($vaeq).conv_tp _
+        exact ($ΓT).inv_el.tp_eq_synthTp.symm_tp.subst ($Δenv).wf_sb
       )⟩
-  | .univ l => return ⟨.univ l,
+  | ~q(.univ $l) => return ⟨q(.univ $l),
       q(by as_aux_lemma =>
         cases ($ΓT).inv_univ
-        have Δ := ($Δenv).wf_sbOfEnv.wf_dom
-        have : $l < univMax := have := ($ΓT).le_univMax; by omega
-        simp only [Expr.subst, Val.toExpr]
-        exact ⟨WfValTp.univ Δ this, EqTp.refl_tp <| WfTp.univ Δ this⟩
+        apply ValEqTp.univ ($Δenv).wf_dom
+        have := ($ΓT).le_univMax
+        omega
       )⟩
-  | A => throw s!"{repr A} is not a type"
+  | A => throwError "{A} is not a type"
 
 /-- Evaluate a term in an environment of values. -/
-partial def evalTm (Δ : Ctx) (env : List Val) (Γ : Ctx) (l : Nat) (t : Expr)
-    (Δenv : Q(WfEnv $Δ $env $Γ))
+partial def evalTm (Δ : Q(Ctx)) (env : Q(List Val)) (σ : Q(Nat → Expr)) (Γ : Q(Ctx))
+    (l : Q(Nat)) (t : Q(Expr))
+    (Δenv : Q(EnvEqSb $Δ $env $σ $Γ))
     (Γt : Q($Γ ⊢[$l] ($t) : synthTp $Γ $t)) :
-    Except String ((v : Val) ×
-      /- Potential simplification: see docstring on `Val`. -/
-      Q(WfValTm $Δ $l $v (synthTp $Γ $t |>.subst (sbOfEnv ‖$Δ‖ $env)) ∧
-        ($Δ ⊢[$l] ($v).toExpr ‖$Δ‖ ≡ ($t).subst (sbOfEnv ‖$Δ‖ $env) :
-          (synthTp $Γ $t |>.subst (sbOfEnv ‖$Δ‖ $env))))) :=
+    Lean.MetaM ((v : Q(Val)) × Q(ValEqTm $Δ $l $v (($t).subst $σ) ((synthTp $Γ $t).subst $σ))) :=
   match t with
-  | .bvar i => do
-    return ⟨env[i]?.getD default,
+  | ~q(.bvar $i) => do
+    let v : Q(Option Val) := q($env[$i]?)
+    /- We evaluate the list access and error if a concrete element doesn't pop out.
+    We do this (instead of producing e.g. `q($env[$i]? |>.getD default)`)
+    because the evaluator may inspect the syntactic form of this value later,
+    and it being `Option.getD ..` would lead to hard-to-debug errors. -/
+    let v : Q(Option Val) ← Lean.Meta.whnf v
+    have pf : $v =Q $env[$i]? := .unsafeIntro -- FIXME: `whnfQ`?
+    let ~q(some $v') := v | throwError "expected 'some _', got{Lean.indentExpr v}"
+    return ⟨v',
       q(by as_aux_lemma =>
+        simp +zetaDelta only [Expr.subst]
         have ⟨_, lk, eq⟩ := ($Γt).inv_bvar
-        simp only [getElem?_pos, ($Δenv).lookup_lt lk, Option.getD_some, Expr.subst,
-          ($Δenv).sbOfEnv_app lk]
-        have iwf := ($Δenv).lookup_wf lk
-        have Δeq := eq.symm_tp.subst ($Δenv).wf_sbOfEnv
-        exact ⟨iwf.conv_nf Δeq, EqTm.refl_tm <| iwf.wf_toExpr.conv Δeq⟩
+        apply ValEqTm.conv_tp _ (eq.subst ($Δenv).wf_sb).symm_tp
+        . convert ($Δenv).lookup_eq lk using 1
+          -- grind -- solves this, but results in `unknown metavariable`
+          subst $v
+          rename_i h
+          have ⟨_, h⟩ := List.getElem?_eq_some_iff.mp h
+          rw [h]
       )⟩
-  | .lam k k' C b => do
-    return ⟨.lam k k' (C.subst (sbOfEnv ‖Δ‖ env)) (.mk_tm Γ C env b),
+  | ~q(.lam $k $k' $C $b) => do
+    return ⟨q(.lam $k $k' (.mk_tm $Γ $C $env $b)),
       q(by as_aux_lemma =>
-        obtain ⟨rfl, D, b, ACD⟩ := ($Γt).inv_lam
-        simp only [synthTp, Expr.subst, Val.toExpr, Clos.toExpr] at ACD ⊢
-        have Δb := (b.subst <| ($Δenv).wf_sbOfEnv.up b.wf_ctx.inv_snoc)
-        constructor
-        . obtain ⟨_, _, _, _, sbD⟩ := ACD.inv_pi
-          apply WfValTm.lam <| WfClosTm.clos_tm
-            (EqTp.refl_tp Δb.wf_ctx.inv_snoc)
-            (sbD.symm_tp.subst <| ($Δenv).wf_sbOfEnv.up b.wf_ctx.inv_snoc)
-            $Δenv
-            b
-        . apply EqTm.conv_eq (EqTm.refl_tm _) (ACD.subst ($Δenv).wf_sbOfEnv).symm_tp
-          apply WfTm.lam Δb
+        simp +zetaDelta only [Expr.subst, synthTp]
+        obtain ⟨rfl, B, b, eq⟩ := ($Γt).inv_lam
+        have C := b.wf_binder
+        apply ValEqTm.lam <| ClosEqTm.clos_tm (B := B) $Δenv _ _ b
+        . exact EqTp.refl_tp <| C.subst ($Δenv).wf_sb
+        . exact b.tp_eq_synthTp.subst (($Δenv).wf_sb.up C)
       )⟩
-  | .app k k' B f a => do
-    let ⟨vf, vfpfs⟩ ← evalTm Δ env Γ (max k k') f
+  | ~q(.app $k $k' $B $f $a) => do
+    let ⟨vf, vfeq⟩ ← evalTm Δ env σ Γ q(max $k $k') f
       q($Δenv)
       q(by as_aux_lemma =>
-        obtain ⟨_, _, f, _⟩ := ($Γt).inv_app
-        apply f.conv f.tp_eq_synthTp
+        have ⟨_, _, f, _⟩ := ($Γt).inv_app
+        exact f.with_synthTp
       )
-    let ⟨va, vapfs⟩ ← evalTm Δ env Γ k a
+    let ⟨va, vaeq⟩ ← evalTm Δ env σ Γ k a
       q($Δenv)
       q(by as_aux_lemma =>
-        obtain ⟨_, _, _, a, _⟩ := ($Γt).inv_app
-        apply a.conv a.tp_eq_synthTp
+        have ⟨_, _, _, a, _⟩ := ($Γt).inv_app
+        exact a.with_synthTp
       )
-    let ⟨v, vpfs⟩ ←
+    let ⟨v, veq⟩ ←
       evalApp Δ k k'
-        (synthTp Γ a |>.subst (sbOfEnv ‖Δ‖ env))
-        (B.subst (Expr.up (sbOfEnv ‖Δ‖ env)))
-        vf
-        va
+        q((synthTp $Γ $a).subst $σ)
+        q(($B).subst (Expr.up $σ))
+        vf va q(($f).subst $σ) q(($a).subst $σ)
         q(by as_aux_lemma =>
-          obtain ⟨_, _, f, a, eq⟩ := ($Γt).inv_app
-          have := EqTp.cong_pi a.tp_eq_synthTp (EqTp.refl_tp f.wf_tp.inv_pi.2)
-            |>.symm_tp.trans_tp f.tp_eq_synthTp
-          apply ($vfpfs).1.conv_nf (this.subst ($Δenv).wf_sbOfEnv).symm_tp
+          apply ($vfeq).conv_tp
+          have ⟨_, _, f, a, _⟩ := ($Γt).inv_app
+          have ⟨_, B⟩ := f.wf_tp.inv_pi
+          apply f.tp_eq_synthTp.subst ($Δenv).wf_sb |>.symm_tp.trans_tp _
+          simp only [Expr.subst]
+          have := a.tp_eq_synthTp.subst ($Δenv).wf_sb
+          gcongr
+          exact B.subst (($Δenv).wf_sb.up B.wf_binder)
         )
-        q(($vapfs).1)
+        q($vaeq)
     return ⟨v,
       q(by as_aux_lemma =>
-        have ⟨vfwf, vfeq⟩ := $vfpfs
-        have ⟨vawf, vaeq⟩ := $vapfs
-        have ⟨vwf, veq⟩ := $vpfs
-        obtain ⟨rfl, _, f, a, _⟩ := ($Γt).inv_app
-        simp only [synthTp, Expr.subst]
-        have BvaBa : $Δ ⊢[$l]
-            (($B).subst (Expr.up (sbOfEnv ‖$Δ‖ $env))).subst (($va).toExpr ‖$Δ‖).toSb ≡
-            (($B).subst ($a).toSb).subst (sbOfEnv ‖$Δ‖ $env) := by
-          have ΓB := f.wf_tp.inv_pi.2.conv_binder a.tp_eq_synthTp
-          have ΔB := ΓB.subst <| ($Δenv).wf_sbOfEnv.up ΓB.wf_ctx.inv_snoc
-          convert ΔB.subst_eq <| EqSb.toSb vaeq using 1; autosubst
-        constructor
-        . exact (vwf).conv_nf BvaBa
-        . apply (veq).trans_tm _ |>.conv_eq BvaBa
-          have sfeq := f.tp_eq_synthTp.subst ($Δenv).wf_sbOfEnv
-          have saeq := a.tp_eq_synthTp.subst ($Δenv).wf_sbOfEnv
-          simp only [Expr.subst] at sfeq saeq
-          have B := f.wf_tp.inv_pi.2
-          apply EqTm.cong_app
-            (EqTp.refl_tp <| B.subst <| ($Δenv).wf_sbOfEnv.up B.wf_ctx.inv_snoc)
-            (vfeq.conv_eq sfeq.symm_tp)
-            (vaeq.conv_eq saeq.symm_tp)
+        obtain ⟨rfl, _, _, _, eq⟩ := ($Γt).inv_app
+        replace eq := eq.subst ($Δenv).wf_sb
+        simp +zetaDelta only [Expr.subst] at eq ⊢
+        apply ($veq).conv_tp
+        convert eq.symm_tp using 1
+        autosubst
       )⟩
-  | .pair k k' B t u => do
-    let ⟨vt, vtpfs⟩ ← evalTm Δ env Γ k t q($Δenv)
+  | ~q(.pair $k $k' $B $t $u) => do
+    let ⟨vt, vteq⟩ ← evalTm Δ env σ Γ k t q($Δenv)
       q(by as_aux_lemma =>
         have ⟨_, _, t, _⟩ := ($Γt).inv_pair
         exact t.with_synthTp)
-    let ⟨vu, vupfs⟩ ← evalTm Δ env Γ k' u q($Δenv)
+    let ⟨vu, vueq⟩ ← evalTm Δ env σ Γ k' u q($Δenv)
       q(by as_aux_lemma =>
         have ⟨_, _, _, u, _⟩ := ($Γt).inv_pair
         exact u.with_synthTp)
-    return ⟨.pair k k' (B.subst <| Expr.up <| sbOfEnv ‖Δ‖ env) vt vu,
+    return ⟨q(.pair $k $k' $vt $vu),
       q(by as_aux_lemma =>
-        have ⟨vtwf, vteq⟩ := $vtpfs
-        have ⟨vuwf, vueq⟩ := $vupfs
-        simp only [synthTp, Expr.subst, Val.toExpr] at ($Γt) ⊢
-        obtain ⟨rfl, _, t, u, eq⟩ := ($Γt).inv_pair
-        have ⟨_, B⟩ := eq.wf_left.inv_sigma
-        have ΔB := B.subst <| ($Δenv).wf_sbOfEnv.up B.wf_ctx.inv_snoc
-        have suenv : $Δ ⊢[$k'] (synthTp $Γ $u).subst (sbOfEnv ‖$Δ‖ $env) ≡
-            (($B).subst (Expr.up (sbOfEnv ‖$Δ‖ $env)) |>.subst (($vt).toExpr ‖$Δ‖).toSb) := by
-          apply u.tp_eq_synthTp.subst ($Δenv).wf_sbOfEnv |>.symm_tp.trans_tp
-          autosubst
-          apply B.subst_eq <| ($Δenv).wf_sbOfEnv.eq_self.snoc t.with_synthTp.wf_tp (vteq).symm_tm
-        constructor
-        . apply WfValTm.pair ΔB vtwf ((vuwf).conv_nf suenv)
-        . apply EqTm.cong_pair (EqTp.refl_tp ΔB) vteq ((vueq).conv_eq suenv)
+        simp +zetaDelta only [synthTp, Expr.subst] at ($Γt) ⊢
+        obtain ⟨rfl, _, _, u, _⟩ := ($Γt).inv_pair
+        have ⟨_, B⟩ := ($Γt).wf_tp.inv_sigma
+        have := B.subst (($Δenv).wf_sb.up B.wf_binder)
+        apply ValEqTm.pair this $vteq
+        apply ($vueq).conv_tp
+        have := u.tp_eq_synthTp.subst ($Δenv).wf_sb
+        convert this.symm_tp using 1; autosubst
       )⟩
-  | .fst l l' A B p => do
-    let ⟨vp, vppfs⟩ ← evalTm Δ env Γ (max l l') p
+  | ~q(.fst $k $k' $A $B $p) => do
+    let ⟨vp, vpeq⟩ ← evalTm Δ env σ Γ q(max $k $k') p
       q($Δenv)
-      q(($Γt).inv_fst.2.1.with_synthTp)
-    let ⟨v, vpfs⟩ ←
-      evalFst Δ l l' (A.subst (sbOfEnv ‖Δ‖ env)) (B.subst (Expr.up (sbOfEnv ‖Δ‖ env))) vp
+      q(by as_aux_lemma => exact ($Γt).inv_fst.2.1.with_synthTp)
+    let ⟨v, veq⟩ ←
+      evalFst Δ k k' q(($A).subst $σ) q(($B).subst (Expr.up $σ)) vp q(($p).subst $σ)
         q(by as_aux_lemma =>
-          have ⟨_, p, eq⟩ := ($Γt).inv_fst
-          have := p.tp_eq_synthTp.subst ($Δenv).wf_sbOfEnv
-          simp only [Expr.subst] at this
-          exact ($vppfs).1.conv_nf this.symm_tp
+          apply ($vpeq).conv_tp
+          have ⟨_, p, _⟩ := ($Γt).inv_fst
+          have := p.tp_eq_synthTp.subst ($Δenv).wf_sb
+          apply this.symm_tp
         )
     return ⟨v,
       q(by as_aux_lemma =>
-        have ⟨_, vpeq⟩ := $vppfs
-        have ⟨vwf, veq⟩ := $vpfs
-        obtain ⟨rfl, p, _⟩ := ($Γt).inv_fst
-        constructor
-        . convert vwf using 1; simp [synthTp]
-        . have eq := p.tp_eq_synthTp.subst ($Δenv).wf_sbOfEnv
-          simp only [Expr.subst, synthTp] at eq ⊢
-          apply veq.trans_tm
-          gcongr
-          apply vpeq.conv_eq eq.symm_tp
+        simp +zetaDelta only [Expr.subst]
+        obtain ⟨rfl, p, eq⟩ := ($Γt).inv_fst
+        apply ($veq).conv_tp (eq.subst ($Δenv).wf_sb).symm_tp
       )⟩
-  | .snd k k' A B p => do
-    let ⟨vp, vppfs⟩ ← evalTm Δ env Γ (max k k') p
+  | ~q(.snd $k $k' $A $B $p) => do
+    let ⟨vp, vpeq⟩ ← evalTm Δ env σ Γ q(max $k $k') p
       q($Δenv)
-      q(($Γt).inv_snd.2.1.with_synthTp)
-    let ⟨v, vpfs⟩ ←
-      evalSnd Δ k k' (A.subst (sbOfEnv ‖Δ‖ env)) (B.subst (Expr.up (sbOfEnv ‖Δ‖ env))) vp
+      q(by as_aux_lemma => exact ($Γt).inv_snd.2.1.with_synthTp)
+    let ⟨v, veq⟩ ←
+      evalSnd Δ k k' q(($A).subst $σ) q(($B).subst (Expr.up $σ)) vp q(($p).subst $σ)
         q(by as_aux_lemma =>
-          have ⟨_, p, eq⟩ := ($Γt).inv_snd
-          have := p.tp_eq_synthTp.subst ($Δenv).wf_sbOfEnv
-          simp only [Expr.subst] at this
-          exact ($vppfs).1.conv_nf this.symm_tp
+          apply ($vpeq).conv_tp
+          have ⟨_, p, _⟩ := ($Γt).inv_snd
+          have := p.tp_eq_synthTp.subst ($Δenv).wf_sb
+          apply this.symm_tp
         )
     return ⟨v,
       q(by as_aux_lemma =>
-        have ⟨_, vpeq⟩ := $vppfs
-        have ⟨vwf, veq⟩ := $vpfs
-        obtain ⟨rfl, p, _⟩ := ($Γt).inv_snd
-        have B := p.wf_tp.inv_sigma.2
-        have speq := p.tp_eq_synthTp.subst ($Δenv).wf_sbOfEnv
-        simp only [synthTp, Expr.subst] at speq ⊢
-        have bigEq : $Δ ⊢[$l]
-              (($B).subst (Expr.up (sbOfEnv ‖$Δ‖ $env)) |>.subst
-                (Expr.fst $k $l
-                  (($A).subst (sbOfEnv ‖$Δ‖ $env))
-                  (($B).subst (Expr.up (sbOfEnv ‖$Δ‖ $env)))
-                  (($vp).toExpr ‖$Δ‖)).toSb) ≡
-              (($B).subst (Expr.fst $k $l $A $B $p).toSb |>.subst (sbOfEnv ‖$Δ‖ $env)) := by
-          autosubst
-          apply B.subst_eq <| ($Δenv).wf_sbOfEnv.eq_self.snoc B.wf_ctx.inv_snoc _
-          gcongr
-          convert vpeq.conv_eq speq.symm_tp using 1; autosubst
-        constructor
-        . apply vwf.conv_nf bigEq
-        . apply EqTm.conv_eq _ bigEq
-          apply veq.trans_tm
-          gcongr
-          apply vpeq.conv_eq speq.symm_tp
+        simp +zetaDelta only [Expr.subst]
+        obtain ⟨rfl, p, eq⟩ := ($Γt).inv_snd
+        apply ($veq).conv_tp
+        convert eq.subst ($Δenv).wf_sb |>.symm_tp using 1
+        autosubst
       )⟩
-  | .code A => do
-    let ⟨vA, vApfs⟩ ← evalTp Δ env Γ (l - 1) A
+  | ~q(.code $A) => do
+    let ⟨vA, vAeq⟩ ← evalTp Δ env σ Γ q($l - 1) A
       q($Δenv)
-      q(by as_aux_lemma => obtain ⟨_, rfl, h, _⟩ := ($Γt).inv_code; exact h
-      )
-    return ⟨.code vA,
+      q(by as_aux_lemma => obtain ⟨_, rfl, h, _⟩ := ($Γt).inv_code; exact h)
+    return ⟨q(.code $vA),
       q(by as_aux_lemma =>
-        have ⟨vAwf, vAeq⟩ := $vApfs
-        simp only [Val.toExpr, Expr.subst, synthTp]
-        obtain ⟨_, rfl, A, _⟩ := ($Γt).inv_code
+        simp +zetaDelta only [Expr.subst]
+        obtain ⟨l, rfl, _, Teq⟩ := ($Γt).inv_code
         have := ($Γt).le_univMax
-        cases A.lvl_eq_synthLvl
-        exact ⟨WfValTm.code (by omega) vAwf, EqTm.cong_code (by omega) vAeq⟩
+        have := Teq.subst ($Δenv).wf_sb
+        apply ValEqTm.conv_tp _ this.symm_tp
+        apply ValEqTm.code (by omega) $vAeq
       )⟩
-  | t => throw s!"{repr t} is not a term"
+  | t => throwError "{t} is not a term"
 
 -- FIXME: `A` could be replaced by `synthTp Δ a`
-partial def evalApp (Δ : Ctx) (l l' : Nat) (A B : Expr) (f a : Val)
-    (Δf : Q(WfValTm $Δ (max $l $l') $f (.pi $l $l' $A $B)))
-    (Δa : Q(WfValTm $Δ $l $a $A)) :
-    Except String ((v : Val) ×
-      Q(WfValTm $Δ $l' $v (($B).subst (($a).toExpr ‖$Δ‖).toSb) ∧
-        ($Δ ⊢[$l'] ($v).toExpr ‖$Δ‖ ≡
-          .app $l $l' $B (($f).toExpr ‖$Δ‖) (($a).toExpr ‖$Δ‖) :
-          (($B).subst (($a).toExpr ‖$Δ‖).toSb)))) :=
-  match f with
-  | .lam m m' _ (.mk_tm Γ A' env b) => do
-    let ⟨v, vpfs⟩ ← evalTm Δ (a :: env) ((A', m) :: Γ) m' b
+partial def evalApp (Δ : Q(Ctx)) (l l' : Q(Nat)) (A B : Q(Expr))
+    (vf va : Q(Val)) (f a : Q(Expr))
+    (Δf : Q(ValEqTm $Δ (max $l $l') $vf $f (.pi $l $l' $A $B)))
+    (Δa : Q(ValEqTm $Δ $l $va $a $A)) :
+    Lean.MetaM ((v : Q(Val)) ×
+      Q(ValEqTm $Δ $l' $v (.app $l $l' $B $f $a) (($B).subst ($a).toSb))) :=
+  match vf with
+  | ~q(.lam $k $k' (.mk_tm $Γ $A' $env $b)) => do
+    /- To evaluate the closure in its environment `env`,
+    we need to provide a substitution `σ` with `EnvEqSb Δ env σ Γ`;
+    but such a substitution is difficult to construct
+    because `Val`s do not contain type annotations whereas `Expr`s do
+    (see now-removed `sbOfEnv`).
+    We also cannot store it in `Clos.mk_tm`
+    because that would make weakening non-free on values.
+    Instead, we obtain one using AC;
+    the choice is unique (up to `EqSb`)
+    since `EnvEqSb` is functional. -/
+    let ex : Q(∃ σ, EnvEqSb $Δ $env σ $Γ) :=
       q(by as_aux_lemma =>
-        have ⟨_, B, b, eq⟩ := ($Δf).inv_lam
-        rcases b with ⟨A'env, _, env, b⟩
-        obtain ⟨_, rfl, rfl, Aeq, _⟩ := eq.inv_pi
-        apply env.snoc b.wf_ctx.inv_snoc (($Δa).conv_nf <| Aeq.trans_tp A'env.symm_tp)
+        have ⟨_, _, _, _, c, _⟩ := ($Δf).inv_lam
+        rcases c with ⟨env, _⟩
+        exact ⟨_, env⟩
+      )
+    let ⟨v, veq⟩ ← evalTm Δ q($va :: $env)
+      q(Expr.snoc (Classical.choose $ex) $a) q(($A', $k) :: $Γ) k' b
+      q(by as_aux_lemma =>
+        have ⟨_, _, _, _, c, eqt, eq⟩ := ($Δf).inv_lam
+        rcases c with ⟨env, Aeq', _, b⟩
+        obtain ⟨_, rfl, rfl, Aeq, Beq⟩ := eq.inv_pi
+        have A' := b.wf_binder
+        apply EnvEqSb.snoc (Classical.choose_spec $ex) A'
+        apply ($Δa).conv_tp <| Aeq.trans_tp <| Aeq'.symm_tp.trans_tp <| A'.subst_eq _
+        exact env.sb_uniq (Classical.choose_spec $ex)
       )
       q(by as_aux_lemma =>
-        have ⟨_, B, b, eq⟩ := ($Δf).inv_lam
-        rcases b with ⟨A'env, _, env, b⟩
+        have ⟨_, _, _, _, c, eqt, eq⟩ := ($Δf).inv_lam
+        rcases c with ⟨_, _, _, b⟩
         exact b.with_synthTp
       )
     return ⟨v,
       q(by as_aux_lemma =>
-        have ⟨vwf, veq⟩ := $vpfs
-        have ⟨_, B, b, eq⟩ := ($Δf).inv_lam
-        rcases b with ⟨A'env, Benv, env, b⟩
+        have ⟨_, _, _, _, c, eqt, eq⟩ := ($Δf).inv_lam
+        rcases c with ⟨env, Aeq', Beq', b⟩
         obtain ⟨_, rfl, rfl, Aeq, Beq⟩ := eq.inv_pi
-        have bigEq : $Δ ⊢[$l'] (synthTp (($A', $l) :: $Γ) $b).subst (sbOfEnv ‖$Δ‖ ($a :: $env)) ≡
-            ($B).subst (Val.toExpr ‖$Δ‖ $a).toSb := by
-          have := b.tp_eq_synthTp.symm_tp.subst (env.wf_sbOfEnv.up b.wf_ctx.inv_snoc)
-            |>.conv_binder (A'env.trans_tp Aeq.symm_tp)
-            |>.trans_tp (Benv.conv_binder Aeq.symm_tp)
-            |>.trans_tp Beq.symm_tp
-          convert this.subst <| WfSb.toSb ($Δa).wf_toExpr using 1
-          autosubst
-          apply sb_irrel.1 b.with_synthTp.wf_tp
-          intro i lt
-          cases i
-          . simp
-          . dsimp; apply sbOfEnv_get_eq; simpa [env.eq_length] using lt
-        constructor
-        . apply vwf.conv_nf bigEq
-        . apply veq.conv_eq bigEq |>.trans_tm
-          have Δb := b.subst (env.wf_sbOfEnv.up b.wf_ctx.inv_snoc)
-            |>.conv_binder A'env |>.conv (Benv.trans_tp <| Beq.symm_tp.conv_binder Aeq)
-          have Δa := ($Δa).conv_nf Aeq
-          simp only [Val.toExpr, Clos.toExpr]
-          convert EqTm.app_lam Δb Δa.wf_toExpr |>.symm_tm.trans_tm _ using 1
-          . autosubst
-            apply sb_irrel.2 b
-            intro i lt
-            cases i
-            . simp
-            . dsimp; apply sbOfEnv_get_eq; simpa [env.eq_length] using lt
-          apply EqTm.refl_tm <| WfTm.app (WfTm.lam Δb) Δa.wf_toExpr
-      )⟩
-  | .neut n => do
-    let n : Val := .neut <| .app l l' B n a
-    return ⟨n,
-      q(by as_aux_lemma =>
-        constructor
-        . exact WfValTm.neut_tm <| WfNeutTm.app ($Δf).inv_neut ($Δa)
-        . simp +zetaDelta only [Val.toExpr, Neut.toExpr]
-          exact EqTm.refl_tm <| WfTm.app ($Δf).inv_neut.wf_toExpr ($Δa).wf_toExpr
-      )⟩
-  | _ => throw s!"unexpected normal form {repr f} at type Π"
+        clear eq
+        have sbeq := env.sb_uniq (Classical.choose_spec $ex)
 
-partial def evalFst (Δ : Ctx) (l l' : Nat) (A B : Expr) (p : Val)
-    (Δp : Q(WfValTm $Δ (max $l $l') $p (.sigma $l $l' $A $B))) :
-    Except String ((v : Val) ×
-      Q(WfValTm $Δ $l $v $A ∧
-        ($Δ ⊢[$l] ($v).toExpr ‖$Δ‖ ≡ .fst $l $l' $A $B (($p).toExpr ‖$Δ‖) : $A))) :=
-  match p with
-  | .pair _ _ _ v _ =>
+        replace sbeq := sbeq.snoc b.wf_binder <| EqTm.refl_tm <| ($Δa).wf_tm.conv <|
+          Aeq.trans_tp Aeq'.symm_tp
+        have := b.tp_eq_synthTp.subst_eq sbeq
+        replace ($veq) := ($veq).conv_nf ((b.subst_eq sbeq).conv_eq this).symm_tm this.symm_tp
+        replace Beq' := Beq'.conv_binder Aeq.symm_tp
+        have := Beq'.trans_tp Beq.symm_tp |>.subst (WfSb.toSb ($Δa).wf_tm)
+        simp only [autosubst] at ($veq) this ⊢
+        apply ($veq).conv_nf _ this
+        apply EqTm.conv_eq _ this.symm_tp
+        replace b := b.subst (env.wf_sb.up b.wf_binder)
+          |>.conv_binder (Aeq'.trans_tp Aeq.symm_tp)
+          |>.conv (Beq'.trans_tp Beq.symm_tp)
+        have := EqTm.app_lam b ($Δa).wf_tm |>.symm_tm
+        simp only [autosubst] at this
+        apply this.trans_tm
+        apply EqTm.cong_app (EqTp.refl_tp Beq.wf_left) _ (EqTm.refl_tm ($Δa).wf_tm)
+        apply EqTm.trans_tm _ eqt.symm_tm
+        gcongr
+        autosubst
+        convert EqTm.refl_tm b using 1 <;> autosubst
+      )⟩
+  | ~q(.neut $n) => do
+    let na : Q(Val) := q(.neut <| .app $l $l' $n $va)
+    return ⟨na,
+      q(by as_aux_lemma =>
+        exact ValEqTm.neut_tm <| NeutEqTm.app ($Δf).inv_neut $Δa
+      )⟩
+  | _ => throwError "unexpected normal form {f} at type Π"
+
+partial def evalFst (Δ : Q(Ctx)) (l l' : Q(Nat)) (A B : Q(Expr))
+    (vp : Q(Val)) (p : Q(Expr))
+    (Δp : Q(ValEqTm $Δ (max $l $l') $vp $p (.sigma $l $l' $A $B))) :
+    Lean.MetaM ((v : Q(Val)) × Q(ValEqTm $Δ $l $v (.fst $l $l' $A $B $p) $A)) :=
+  match vp with
+  | ~q(.pair _ _ $v _) =>
     return ⟨v,
       q(by as_aux_lemma =>
-        simp only [Val.toExpr]
-        have ⟨_, _, v, w, eq⟩ := ($Δp).inv_pair
+        have ⟨_, A', B', f, s, v, _, eqt, eq⟩ := ($Δp).inv_pair
         obtain ⟨_, rfl, rfl, Aeq, Beq⟩ := eq.inv_sigma
-        replace v := v.conv_nf Aeq.symm_tp
-        refine ⟨v, ?_⟩
-        apply EqTm.fst_pair Beq.wf_right v.wf_toExpr w.wf_toExpr |>.symm_tm.trans_tm
-        gcongr
-        apply WfTm.pair Beq.wf_right v.wf_toExpr w.wf_toExpr
+        have : $Δ ⊢[$l] f ≡ Expr.fst $l $l' $A $B $p : $A := by
+          have ⟨_, A'', t, u, eq'⟩ := eqt.wf_right.inv_pair
+          have ⟨_, _, _, Aeq', Beq'⟩ := eq'.inv_sigma
+          replace t := t.conv Aeq'.symm_tp
+          replace u := u.conv <| Beq'.symm_tp.subst (WfSb.toSb t)
+          apply EqTm.fst_pair Beq.wf_left t u |>.symm_tm.trans_tm
+          gcongr
+          apply EqTm.trans_tm _ eqt.symm_tm
+          gcongr <;> assumption
+        apply v.conv_nf (this.conv_eq Aeq) Aeq.symm_tp
       )⟩
-  | .neut n =>
-    return ⟨.neut (.fst l l' A B n),
+  | ~q(.neut $n) =>
+    return ⟨q(.neut (.fst $l $l' $n)),
       q(by as_aux_lemma =>
-        constructor
-        . exact WfValTm.neut_tm <| WfNeutTm.fst ($Δp).inv_neut
-        . convert EqTm.refl_tm <| WfTm.fst ($Δp).wf_toExpr using 1
-          simp [Val.toExpr, Neut.toExpr]
+        exact ValEqTm.neut_tm <| NeutEqTm.fst ($Δp).inv_neut
       )⟩
-  | _ => throw s!"unexpected normal form {repr p} at type Σ"
+  | _ => throwError "unexpected normal form {p} at type Σ"
 
-partial def evalSnd (Δ : Ctx) (l l' : Nat) (A B : Expr) (p : Val)
-    (Δp : Q(WfValTm $Δ (max $l $l') $p (.sigma $l $l' $A $B))) :
-    Except String ((v : Val) ×
-      Q(WfValTm $Δ $l' $v (($B).subst (Expr.fst $l $l' $A $B (($p).toExpr ‖$Δ‖)).toSb) ∧
-        ($Δ ⊢[$l'] ($v).toExpr ‖$Δ‖ ≡ .snd $l $l' $A $B (($p).toExpr ‖$Δ‖) :
-          ($B).subst (Expr.fst $l $l' $A $B (($p).toExpr ‖$Δ‖)).toSb))) :=
-  match p with
-  | .pair _ _ B' v w =>
+partial def evalSnd (Δ : Q(Ctx)) (l l' : Q(Nat)) (A B : Q(Expr))
+    (vp : Q(Val)) (p : Q(Expr))
+    (Δp : Q(ValEqTm $Δ (max $l $l') $vp $p (.sigma $l $l' $A $B))) :
+    Lean.MetaM ((v : Q(Val)) ×
+      Q(ValEqTm $Δ $l' $v (.snd $l $l' $A $B $p) <| ($B).subst (Expr.fst $l $l' $A $B $p).toSb)) :=
+  match vp with
+  | ~q(.pair _ _ _ $w) =>
     return ⟨w,
       q(by as_aux_lemma =>
-        simp only [Val.toExpr]
-        have ⟨_, _, v, w, eq⟩ := ($Δp).inv_pair
-        obtain ⟨_, rfl, rfl, Aeq,Beq⟩ := eq.inv_sigma
-        replace v := v.conv_nf Aeq.symm_tp
-        have fstPair : $Δ ⊢[$l]
-            (Expr.fst $l $l' $A $B (Expr.pair $l $l' $B' (($v).toExpr ‖$Δ‖) (($w).toExpr ‖$Δ‖))) ≡
-              (($v).toExpr ‖$Δ‖) : $A := by
-          apply EqTm.trans_tm _ <| EqTm.fst_pair Beq.wf_right v.wf_toExpr w.wf_toExpr
+        have ⟨_, A', B', f, s, _, w, eqt, eq⟩ := ($Δp).inv_pair
+        obtain ⟨_, rfl, rfl, Aeq, Beq⟩ := eq.inv_sigma
+        have ⟨_, A'', t, u, eq'⟩ := eqt.wf_right.inv_pair
+        have ⟨_, _, _, Aeq', Beq'⟩ := eq'.inv_sigma
+        replace t := t.conv Aeq'.symm_tp
+        replace u := u.conv <| Beq'.symm_tp.subst (WfSb.toSb t)
+        have feq : $Δ ⊢[$l] f ≡ Expr.fst $l $l' $A $B $p : $A := by
+          apply EqTm.fst_pair Beq.wf_left t u |>.symm_tm.trans_tm
           gcongr
-          apply WfTm.pair Beq.wf_right v.wf_toExpr w.wf_toExpr |>.conv
-          gcongr
-        have BFstPair := Beq.symm_tp.subst_eq <| EqSb.toSb fstPair.symm_tm
-        constructor
-        . apply w.conv_nf BFstPair
-        . have := EqTm.snd_pair Beq.wf_right v.wf_toExpr w.wf_toExpr |>.symm_tm
-          apply this.conv_eq BFstPair |>.trans_tm
-          symm; gcongr
-          apply WfTm.pair Beq.wf_right v.wf_toExpr w.wf_toExpr |>.conv
-          gcongr
+          apply EqTm.trans_tm _ eqt.symm_tm
+          gcongr <;> assumption
+        replace w := w.conv_tp <| Beq.symm_tp.subst_eq (EqSb.toSb feq)
+        apply w.conv_nf _ (EqTp.refl_tp w.wf_tm.wf_tp)
+        apply EqTm.snd_pair Beq.wf_left t u |>.symm_tm.conv_eq
+          (Beq'.wf_left.subst_eq (EqSb.toSb feq)) |>.trans_tm _
+        symm; gcongr
+        apply eqt.trans_tm
+        symm; gcongr <;> assumption
       )⟩
-  | .neut n =>
-    return ⟨.neut (.snd l l' A B n),
+  | ~q(.neut $n) =>
+    return ⟨q(.neut (.snd $l $l' $n)),
       q(by as_aux_lemma =>
-        simp only [Val.toExpr, Neut.toExpr]
-        constructor
-        . exact WfValTm.neut_tm <| WfNeutTm.snd ($Δp).inv_neut
-        . convert EqTm.refl_tm <| WfTm.snd ($Δp).wf_toExpr using 1 <;> simp [Val.toExpr]
+        exact ValEqTm.neut_tm <| NeutEqTm.snd ($Δp).inv_neut
       )⟩
-  | _ => throw s!"unexpected normal form {repr p} at type Σ"
+  | _ => throwError "unexpected normal form {p} at type Σ"
 
 end
